new/code/github_com/goose_lang/goose/testdata/examples/semantics.v
@@ -499,15 +499,15 @@ Definition roundtripEncDec32 : val :=
     let: "$r0" := (slice.make2 byteT #(W64 4)) in
     do:  ("r" <-[sliceT] "$r0");;;
     let: "e" := (ref_ty ptrT (zero_val ptrT)) in
-    let: "$r0" := (ref_ty Enc (let: "p" := (![sliceT] "r") in
+    let: "$r0" := (ref_ty Enc (let: "$p" := (![sliceT] "r") in
     struct.make Enc [{
-      "p" ::= "p"
+      "p" ::= "$p"
     }])) in
     do:  ("e" <-[ptrT] "$r0");;;
     let: "d" := (ref_ty ptrT (zero_val ptrT)) in
-    let: "$r0" := (ref_ty Dec (let: "p" := (![sliceT] "r") in
+    let: "$r0" := (ref_ty Dec (let: "$p" := (![sliceT] "r") in
     struct.make Dec [{
-      "p" ::= "p"
+      "p" ::= "$p"
     }])) in
     do:  ("d" <-[ptrT] "$r0");;;
     do:  (let: "$a0" := (let: "$a0" := #(W64 4) in
@@ -526,15 +526,15 @@ Definition roundtripEncDec64 : val :=
     let: "$r0" := (slice.make2 byteT #(W64 8)) in
     do:  ("r" <-[sliceT] "$r0");;;
     let: "e" := (ref_ty ptrT (zero_val ptrT)) in
-    let: "$r0" := (ref_ty Enc (let: "p" := (![sliceT] "r") in
+    let: "$r0" := (ref_ty Enc (let: "$p" := (![sliceT] "r") in
     struct.make Enc [{
-      "p" ::= "p"
+      "p" ::= "$p"
     }])) in
     do:  ("e" <-[ptrT] "$r0");;;
     let: "d" := (ref_ty ptrT (zero_val ptrT)) in
-    let: "$r0" := (ref_ty Dec (let: "p" := (![sliceT] "r") in
+    let: "$r0" := (ref_ty Dec (let: "$p" := (![sliceT] "r") in
     struct.make Dec [{
-      "p" ::= "p"
+      "p" ::= "$p"
     }])) in
     do:  ("d" <-[ptrT] "$r0");;;
     do:  (let: "$a0" := (let: "$a0" := #(W64 8) in
@@ -724,21 +724,21 @@ Definition failing_testFunctionOrdering : val :=
     let: "$r0" := (slice.make2 uint64T #(W64 5)) in
     do:  ("arr" <-[sliceT] "$r0");;;
     let: "e1" := (ref_ty Editor (zero_val Editor)) in
-    let: "$r0" := (let: "s" := (let: "$s" := (![sliceT] "arr") in
+    let: "$r0" := (let: "$s" := (let: "$s" := (![sliceT] "arr") in
     slice.slice uint64T "$s" #(W64 0) (slice.len "$s")) in
-    let: "next_val" := #(W64 1) in
+    let: "$next_val" := #(W64 1) in
     struct.make Editor [{
-      "s" ::= "s";
-      "next_val" ::= "next_val"
+      "s" ::= "$s";
+      "next_val" ::= "$next_val"
     }]) in
     do:  ("e1" <-[Editor] "$r0");;;
     let: "e2" := (ref_ty Editor (zero_val Editor)) in
-    let: "$r0" := (let: "s" := (let: "$s" := (![sliceT] "arr") in
+    let: "$r0" := (let: "$s" := (let: "$s" := (![sliceT] "arr") in
     slice.slice uint64T "$s" #(W64 0) (slice.len "$s")) in
-    let: "next_val" := #(W64 101) in
+    let: "$next_val" := #(W64 101) in
     struct.make Editor [{
-      "s" ::= "s";
-      "next_val" ::= "next_val"
+      "s" ::= "$s";
+      "next_val" ::= "$next_val"
     }]) in
     do:  ("e2" <-[Editor] "$r0");;;
     (if: ((let: "$a0" := #(W64 2) in
@@ -767,26 +767,26 @@ Definition failing_testFunctionOrdering : val :=
     then return: (#false)
     else do:  #());;;
     let: "p" := (ref_ty Pair (zero_val Pair)) in
-    let: "$r0" := (let: "x" := (let: "$a0" := #(W64 5) in
+    let: "$r0" := (let: "$x" := (let: "$a0" := #(W64 5) in
     (Editor__AdvanceReturn "e1") "$a0") in
-    let: "y" := (let: "$a0" := #(W64 105) in
+    let: "$y" := (let: "$a0" := #(W64 105) in
     (Editor__AdvanceReturn "e2") "$a0") in
     struct.make Pair [{
-      "x" ::= "x";
-      "y" ::= "y"
+      "x" ::= "$x";
+      "y" ::= "$y"
     }]) in
     do:  ("p" <-[Pair] "$r0");;;
     (if: (![uint64T] (slice.elem_ref uint64T (![sliceT] "arr") #(W64 3))) ≠ #(W64 104)
     then return: (#false)
     else do:  #());;;
     let: "q" := (ref_ty Pair (zero_val Pair)) in
-    let: "$r0" := (let: "y" := (let: "$a0" := #(W64 6) in
+    let: "$r0" := (let: "$y" := (let: "$a0" := #(W64 6) in
     (Editor__AdvanceReturn "e1") "$a0") in
-    let: "x" := (let: "$a0" := #(W64 106) in
+    let: "$x" := (let: "$a0" := #(W64 106) in
     (Editor__AdvanceReturn "e2") "$a0") in
     struct.make Pair [{
-      "x" ::= "x";
-      "y" ::= "y"
+      "x" ::= "$x";
+      "y" ::= "$y"
     }]) in
     do:  ("q" <-[Pair] "$r0");;;
     (if: (![uint64T] (slice.elem_ref uint64T (![sliceT] "arr") #(W64 4))) ≠ #(W64 105)
@@ -891,17 +891,17 @@ Definition testGenericStructs : val :=
     let: "$r0" := #(W64 2) in
     do:  (map.insert (![IntMap uint64T] "intMap") #(W64 1) "$r0");;;
     let: "c" := (ref_ty (genericStruct2 uint64T) (zero_val (genericStruct2 uint64T))) in
-    let: "$r0" := (let: "g" := #(W64 2) in
+    let: "$r0" := (let: "$g" := #(W64 2) in
     struct.make (genericStruct2 uint64T) [{
-      "g" ::= "g"
+      "g" ::= "$g"
     }]) in
     do:  ("c" <-[genericStruct2 uint64T] "$r0");;;
     let: "u" := (ref_ty (genericStruct stringT uint64T) (zero_val (genericStruct stringT uint64T))) in
-    let: "$r0" := (let: "x" := #"test" in
-    let: "y" := #(W64 7) in
+    let: "$r0" := (let: "$x" := #"test" in
+    let: "$y" := #(W64 7) in
     struct.make (genericStruct stringT uint64T) [{
-      "x" ::= "x";
-      "y" ::= "y"
+      "x" ::= "$x";
+      "y" ::= "$y"
     }]) in
     do:  ("u" <-[genericStruct stringT uint64T] "$r0");;;
     let: "d" := (ref_ty uint64T (zero_val uint64T)) in
@@ -928,9 +928,9 @@ Definition testGenericStructs : val :=
     do:  "$r0";;;
     do:  ("b" <-[uint64T] "$r1");;;
     let: "h" := (ref_ty nonGenericStruct (zero_val nonGenericStruct)) in
-    let: "$r0" := (let: "p" := #(W64 3) in
+    let: "$r0" := (let: "$p" := #(W64 3) in
     struct.make nonGenericStruct [{
-      "p" ::= "p"
+      "p" ::= "$p"
     }]) in
     do:  ("h" <-[nonGenericStruct] "$r0");;;
     return: ((((((((![uint64T] "d") + (![uint64T] "d2")) + (![uint64T] (struct.field_ref (genericStruct2 uint64T) "g" "c"))) + (![uint64T] (struct.field_ref (genericStruct stringT uint64T) "y" "u"))) + (![uint64T] "b")) + (![uint64T] (struct.field_ref nonGenericStruct "p" "h"))) + (Fst (map.get (![IntMap uint64T] "intMap") #(W64 1)))) = #(W64 27))).
@@ -1037,9 +1037,9 @@ Definition SquareStruct__mset_ptr : list (string * val) := [
 Definition testBasicInterface : val :=
   rec: "testBasicInterface" <> :=
     exception_do (let: "s" := (ref_ty SquareStruct (zero_val SquareStruct)) in
-    let: "$r0" := (let: "Side" := #(W64 2) in
+    let: "$r0" := (let: "$Side" := #(W64 2) in
     struct.make SquareStruct [{
-      "Side" ::= "Side"
+      "Side" ::= "$Side"
     }]) in
     do:  ("s" <-[SquareStruct] "$r0");;;
     return: ((let: "$a0" := (interface.make SquareStruct__mset (![SquareStruct] "s")) in
@@ -1049,9 +1049,9 @@ Definition testBasicInterface : val :=
 Definition testAssignInterface : val :=
   rec: "testAssignInterface" <> :=
     exception_do (let: "s" := (ref_ty SquareStruct (zero_val SquareStruct)) in
-    let: "$r0" := (let: "Side" := #(W64 3) in
+    let: "$r0" := (let: "$Side" := #(W64 3) in
     struct.make SquareStruct [{
-      "Side" ::= "Side"
+      "Side" ::= "$Side"
     }]) in
     do:  ("s" <-[SquareStruct] "$r0");;;
     let: "area" := (ref_ty uint64T (zero_val uint64T)) in
@@ -1064,9 +1064,9 @@ Definition testAssignInterface : val :=
 Definition testMultipleInterface : val :=
   rec: "testMultipleInterface" <> :=
     exception_do (let: "s" := (ref_ty SquareStruct (zero_val SquareStruct)) in
-    let: "$r0" := (let: "Side" := #(W64 3) in
+    let: "$r0" := (let: "$Side" := #(W64 3) in
     struct.make SquareStruct [{
-      "Side" ::= "Side"
+      "Side" ::= "$Side"
     }]) in
     do:  ("s" <-[SquareStruct] "$r0");;;
     let: "square1" := (ref_ty uint64T (zero_val uint64T)) in
@@ -1083,9 +1083,9 @@ Definition testMultipleInterface : val :=
 Definition testBinaryExprInterface : val :=
   rec: "testBinaryExprInterface" <> :=
     exception_do (let: "s" := (ref_ty SquareStruct (zero_val SquareStruct)) in
-    let: "$r0" := (let: "Side" := #(W64 3) in
+    let: "$r0" := (let: "$Side" := #(W64 3) in
     struct.make SquareStruct [{
-      "Side" ::= "Side"
+      "Side" ::= "$Side"
     }]) in
     do:  ("s" <-[SquareStruct] "$r0");;;
     let: "square1" := (ref_ty uint64T (zero_val uint64T)) in
@@ -1104,9 +1104,9 @@ Definition testBinaryExprInterface : val :=
 Definition testIfStmtInterface : val :=
   rec: "testIfStmtInterface" <> :=
     exception_do (let: "s" := (ref_ty SquareStruct (zero_val SquareStruct)) in
-    let: "$r0" := (let: "Side" := #(W64 3) in
+    let: "$r0" := (let: "$Side" := #(W64 3) in
     struct.make SquareStruct [{
-      "Side" ::= "Side"
+      "Side" ::= "$Side"
     }]) in
     do:  ("s" <-[SquareStruct] "$r0");;;
     (if: (let: "$a0" := (interface.make SquareStruct__mset (![SquareStruct] "s")) in
@@ -1211,9 +1211,9 @@ Definition testStandardForLoop : val :=
 Definition testForLoopWait : val :=
   rec: "testForLoopWait" <> :=
     exception_do (let: "ls" := (ref_ty LoopStruct (zero_val LoopStruct)) in
-    let: "$r0" := (let: "loopNext" := (ref_ty uint64T (zero_val uint64T)) in
+    let: "$r0" := (let: "$loopNext" := (ref_ty uint64T (zero_val uint64T)) in
     struct.make LoopStruct [{
-      "loopNext" ::= "loopNext"
+      "loopNext" ::= "$loopNext"
     }]) in
     do:  ("ls" <-[LoopStruct] "$r0");;;
     do:  (let: "$a0" := #(W64 3) in
@@ -1951,15 +1951,15 @@ Definition CheckFalse : val :=
 Definition testShortcircuitAndTF : val :=
   rec: "testShortcircuitAndTF" <> :=
     exception_do (let: "b" := (ref_ty ptrT (zero_val ptrT)) in
-    let: "$r0" := (ref_ty BoolTest (let: "t" := #true in
-    let: "f" := #false in
-    let: "tc" := #(W64 0) in
-    let: "fc" := #(W64 0) in
+    let: "$r0" := (ref_ty BoolTest (let: "$t" := #true in
+    let: "$f" := #false in
+    let: "$tc" := #(W64 0) in
+    let: "$fc" := #(W64 0) in
     struct.make BoolTest [{
-      "t" ::= "t";
-      "f" ::= "f";
-      "tc" ::= "tc";
-      "fc" ::= "fc"
+      "t" ::= "$t";
+      "f" ::= "$f";
+      "tc" ::= "$tc";
+      "fc" ::= "$fc"
     }])) in
     do:  ("b" <-[ptrT] "$r0");;;
     (if: (let: "$a0" := (![ptrT] "b") in
@@ -1973,15 +1973,15 @@ Definition testShortcircuitAndTF : val :=
 Definition testShortcircuitAndFT : val :=
   rec: "testShortcircuitAndFT" <> :=
     exception_do (let: "b" := (ref_ty ptrT (zero_val ptrT)) in
-    let: "$r0" := (ref_ty BoolTest (let: "t" := #true in
-    let: "f" := #false in
-    let: "tc" := #(W64 0) in
-    let: "fc" := #(W64 0) in
+    let: "$r0" := (ref_ty BoolTest (let: "$t" := #true in
+    let: "$f" := #false in
+    let: "$tc" := #(W64 0) in
+    let: "$fc" := #(W64 0) in
     struct.make BoolTest [{
-      "t" ::= "t";
-      "f" ::= "f";
-      "tc" ::= "tc";
-      "fc" ::= "fc"
+      "t" ::= "$t";
+      "f" ::= "$f";
+      "tc" ::= "$tc";
+      "fc" ::= "$fc"
     }])) in
     do:  ("b" <-[ptrT] "$r0");;;
     (if: (let: "$a0" := (![ptrT] "b") in
@@ -1995,15 +1995,15 @@ Definition testShortcircuitAndFT : val :=
 Definition testShortcircuitOrTF : val :=
   rec: "testShortcircuitOrTF" <> :=
     exception_do (let: "b" := (ref_ty ptrT (zero_val ptrT)) in
-    let: "$r0" := (ref_ty BoolTest (let: "t" := #true in
-    let: "f" := #false in
-    let: "tc" := #(W64 0) in
-    let: "fc" := #(W64 0) in
+    let: "$r0" := (ref_ty BoolTest (let: "$t" := #true in
+    let: "$f" := #false in
+    let: "$tc" := #(W64 0) in
+    let: "$fc" := #(W64 0) in
     struct.make BoolTest [{
-      "t" ::= "t";
-      "f" ::= "f";
-      "tc" ::= "tc";
-      "fc" ::= "fc"
+      "t" ::= "$t";
+      "f" ::= "$f";
+      "tc" ::= "$tc";
+      "fc" ::= "$fc"
     }])) in
     do:  ("b" <-[ptrT] "$r0");;;
     (if: (let: "$a0" := (![ptrT] "b") in
@@ -2017,15 +2017,15 @@ Definition testShortcircuitOrTF : val :=
 Definition testShortcircuitOrFT : val :=
   rec: "testShortcircuitOrFT" <> :=
     exception_do (let: "b" := (ref_ty ptrT (zero_val ptrT)) in
-    let: "$r0" := (ref_ty BoolTest (let: "t" := #true in
-    let: "f" := #false in
-    let: "tc" := #(W64 0) in
-    let: "fc" := #(W64 0) in
+    let: "$r0" := (ref_ty BoolTest (let: "$t" := #true in
+    let: "$f" := #false in
+    let: "$tc" := #(W64 0) in
+    let: "$fc" := #(W64 0) in
     struct.make BoolTest [{
-      "t" ::= "t";
-      "f" ::= "f";
-      "tc" ::= "tc";
-      "fc" ::= "fc"
+      "t" ::= "$t";
+      "f" ::= "$f";
+      "tc" ::= "$tc";
+      "fc" ::= "$fc"
     }])) in
     do:  ("b" <-[ptrT] "$r0");;;
     (if: (let: "$a0" := (![ptrT] "b") in
@@ -2161,21 +2161,21 @@ Definition testOverwriteArray : val :=
     let: "$r0" := (slice.make2 uint64T #(W64 4)) in
     do:  ("arr" <-[sliceT] "$r0");;;
     let: "ae1" := (ref_ty ptrT (zero_val ptrT)) in
-    let: "$r0" := (ref_ty ArrayEditor (let: "s" := (let: "$s" := (![sliceT] "arr") in
+    let: "$r0" := (ref_ty ArrayEditor (let: "$s" := (let: "$s" := (![sliceT] "arr") in
     slice.slice uint64T "$s" #(W64 0) (slice.len "$s")) in
-    let: "next_val" := #(W64 1) in
+    let: "$next_val" := #(W64 1) in
     struct.make ArrayEditor [{
-      "s" ::= "s";
-      "next_val" ::= "next_val"
+      "s" ::= "$s";
+      "next_val" ::= "$next_val"
     }])) in
     do:  ("ae1" <-[ptrT] "$r0");;;
     let: "ae2" := (ref_ty ptrT (zero_val ptrT)) in
-    let: "$r0" := (ref_ty ArrayEditor (let: "s" := (let: "$s" := (![sliceT] "arr") in
+    let: "$r0" := (ref_ty ArrayEditor (let: "$s" := (let: "$s" := (![sliceT] "arr") in
     slice.slice uint64T "$s" #(W64 1) (slice.len "$s")) in
-    let: "next_val" := #(W64 102) in
+    let: "$next_val" := #(W64 102) in
     struct.make ArrayEditor [{
-      "s" ::= "s";
-      "next_val" ::= "next_val"
+      "s" ::= "$s";
+      "next_val" ::= "$next_val"
     }])) in
     do:  ("ae2" <-[ptrT] "$r0");;;
     do:  (let: "$a0" := (![sliceT] "arr") in
@@ -2269,14 +2269,14 @@ Definition Foo__mset_ptr : list (string * val) := [
 Definition failing_testFooBarMutation : val :=
   rec: "failing_testFooBarMutation" <> :=
     exception_do (let: "x" := (ref_ty Foo (zero_val Foo)) in
-    let: "$r0" := (let: "bar" := (let: "a" := #(W64 0) in
-    let: "b" := #(W64 0) in
+    let: "$r0" := (let: "$bar" := (let: "$a" := #(W64 0) in
+    let: "$b" := #(W64 0) in
     struct.make Bar [{
-      "a" ::= "a";
-      "b" ::= "b"
+      "a" ::= "$a";
+      "b" ::= "$b"
     }]) in
     struct.make Foo [{
-      "bar" ::= "bar"
+      "bar" ::= "$bar"
     }]) in
     do:  ("x" <-[Foo] "$r0");;;
     do:  ((Foo__mutateBar "x") #());;;
@@ -2349,18 +2349,18 @@ Definition S__mset_ptr : list (string * val) := [
 (* go: structs.go:14:6 *)
 Definition NewS : val :=
   rec: "NewS" <> :=
-    exception_do (return: (ref_ty S (let: "a" := #(W64 2) in
-     let: "b" := (let: "x" := #(W64 1) in
-     let: "y" := #(W64 2) in
+    exception_do (return: (ref_ty S (let: "$a" := #(W64 2) in
+     let: "$b" := (let: "$x" := #(W64 1) in
+     let: "$y" := #(W64 2) in
      struct.make TwoInts [{
-       "x" ::= "x";
-       "y" ::= "y"
+       "x" ::= "$x";
+       "y" ::= "$y"
      }]) in
-     let: "c" := #true in
+     let: "$c" := #true in
      struct.make S [{
-       "a" ::= "a";
-       "b" ::= "b";
-       "c" ::= "c"
+       "a" ::= "$a";
+       "b" ::= "$b";
+       "c" ::= "$c"
      }]))).
 
 (* go: structs.go:42:6 *)
@@ -2449,19 +2449,19 @@ Definition testStructConstructions : val :=
     let: "p1" := (ref_ty ptrT (zero_val ptrT)) in
     let: "p2" := (ref_ty TwoInts (zero_val TwoInts)) in
     let: "p3" := (ref_ty TwoInts (zero_val TwoInts)) in
-    let: "$r0" := (let: "y" := #(W64 0) in
-    let: "x" := #(W64 0) in
+    let: "$r0" := (let: "$y" := #(W64 0) in
+    let: "$x" := #(W64 0) in
     struct.make TwoInts [{
-      "x" ::= "x";
-      "y" ::= "y"
+      "x" ::= "$x";
+      "y" ::= "$y"
     }]) in
     do:  ("p3" <-[TwoInts] "$r0");;;
     let: "p4" := (ref_ty TwoInts (zero_val TwoInts)) in
-    let: "$r0" := (let: "x" := #(W64 0) in
-    let: "y" := #(W64 0) in
+    let: "$r0" := (let: "$x" := #(W64 0) in
+    let: "$y" := #(W64 0) in
     struct.make TwoInts [{
-      "x" ::= "x";
-      "y" ::= "y"
+      "x" ::= "$x";
+      "y" ::= "$y"
     }]) in
     do:  ("p4" <-[TwoInts] "$r0");;;
     let: "$r0" := ((![boolT] "ok") && ((![ptrT] "p1") = #null)) in
@@ -2485,18 +2485,18 @@ Definition testIncompleteStruct : val :=
     let: "$r0" := #true in
     do:  ("ok" <-[boolT] "$r0");;;
     let: "p1" := (ref_ty TwoInts (zero_val TwoInts)) in
-    let: "$r0" := (let: "x" := #(W64 0) in
+    let: "$r0" := (let: "$x" := #(W64 0) in
     struct.make TwoInts [{
-      "x" ::= "x";
+      "x" ::= "$x";
       "y" ::= zero_val uint64T
     }]) in
     do:  ("p1" <-[TwoInts] "$r0");;;
     let: "$r0" := ((![boolT] "ok") && ((![uint64T] (struct.field_ref TwoInts "y" "p1")) = #(W64 0))) in
     do:  ("ok" <-[boolT] "$r0");;;
     let: "p2" := (ref_ty S (zero_val S)) in
-    let: "$r0" := (let: "a" := #(W64 2) in
+    let: "$r0" := (let: "$a" := #(W64 2) in
     struct.make S [{
-      "a" ::= "a";
+      "a" ::= "$a";
       "b" ::= zero_val TwoInts;
       "c" ::= zero_val boolT
     }]) in
@@ -2521,9 +2521,9 @@ Definition StructWrap__mset_ptr : list (string * val) := [
 Definition testStoreInStructVar : val :=
   rec: "testStoreInStructVar" <> :=
     exception_do (let: "p" := (ref_ty StructWrap (zero_val StructWrap)) in
-    let: "$r0" := (let: "i" := #(W64 0) in
+    let: "$r0" := (let: "$i" := #(W64 0) in
     struct.make StructWrap [{
-      "i" ::= "i"
+      "i" ::= "$i"
     }]) in
     do:  ("p" <-[StructWrap] "$r0");;;
     let: "$r0" := #(W64 5) in
@@ -2546,11 +2546,11 @@ Definition testStoreComposite : val :=
     exception_do (let: "p" := (ref_ty ptrT (zero_val ptrT)) in
     let: "$r0" := (ref_ty TwoInts (zero_val TwoInts)) in
     do:  ("p" <-[ptrT] "$r0");;;
-    let: "$r0" := (let: "x" := #(W64 3) in
-    let: "y" := #(W64 4) in
+    let: "$r0" := (let: "$x" := #(W64 3) in
+    let: "$y" := #(W64 4) in
     struct.make TwoInts [{
-      "x" ::= "x";
-      "y" ::= "y"
+      "x" ::= "$x";
+      "y" ::= "$y"
     }]) in
     do:  ((![ptrT] "p") <-[TwoInts] "$r0");;;
     return: ((![uint64T] (struct.field_ref TwoInts "y" (![ptrT] "p"))) = #(W64 4))).
@@ -3019,15 +3019,15 @@ Definition New : val :=
     let: "l" := (ref_ty ptrT (zero_val ptrT)) in
     let: "$r0" := (ref_ty sync.Mutex (zero_val sync.Mutex)) in
     do:  ("l" <-[ptrT] "$r0");;;
-    return: (let: "d" := (![disk.Disk] "d") in
-     let: "cache" := (![mapT uint64T sliceT] "cache") in
-     let: "length" := (![ptrT] "lengthPtr") in
-     let: "l" := (![ptrT] "l") in
+    return: (let: "$d" := (![disk.Disk] "d") in
+     let: "$cache" := (![mapT uint64T sliceT] "cache") in
+     let: "$length" := (![ptrT] "lengthPtr") in
+     let: "$l" := (![ptrT] "l") in
      struct.make Log [{
-       "d" ::= "d";
-       "l" ::= "l";
-       "cache" ::= "cache";
-       "length" ::= "length"
+       "d" ::= "$d";
+       "l" ::= "$l";
+       "cache" ::= "$cache";
+       "length" ::= "$length"
      }])).
 
 (* Open recovers the log following a crash or shutdown
@@ -3062,15 +3062,15 @@ Definition Open : val :=
     let: "l" := (ref_ty ptrT (zero_val ptrT)) in
     let: "$r0" := (ref_ty sync.Mutex (zero_val sync.Mutex)) in
     do:  ("l" <-[ptrT] "$r0");;;
-    return: (let: "d" := (![disk.Disk] "d") in
-     let: "cache" := (![mapT uint64T sliceT] "cache") in
-     let: "length" := (![ptrT] "lengthPtr") in
-     let: "l" := (![ptrT] "l") in
+    return: (let: "$d" := (![disk.Disk] "d") in
+     let: "$cache" := (![mapT uint64T sliceT] "cache") in
+     let: "$length" := (![ptrT] "lengthPtr") in
+     let: "$l" := (![ptrT] "l") in
      struct.make Log [{
-       "d" ::= "d";
-       "l" ::= "l";
-       "cache" ::= "cache";
-       "length" ::= "length"
+       "d" ::= "$d";
+       "l" ::= "$l";
+       "cache" ::= "$cache";
+       "length" ::= "$length"
      }])).
 
 (* disabled since performance is quite poor
