new/code/go_etcd_io/raft/v3.v
@@ -339,12 +339,12 @@ Definition raft__maybeSendSnapshot : val :=
     let: "$sl2" := (interface.make tracker.Progress__mset_ptr (![ptrT] "pr")) in
     slice.literal interfaceT ["$sl0"; "$sl1"; "$sl2"])) in
     (interface.get "Debugf" (![Logger] (struct.field_ref raft "logger" (![ptrT] "r")))) "$a0" "$a1");;;
-    do:  (let: "$a0" := (let: "To" := (![uint64T] "to") in
-    let: "Type" := raftpb.MsgSnap in
-    let: "Snapshot" := "snapshot" in
+    do:  (let: "$a0" := (let: "$To" := (![uint64T] "to") in
+    let: "$Type" := raftpb.MsgSnap in
+    let: "$Snapshot" := "snapshot" in
     struct.make raftpb.Message [{
-      "Type" ::= "Type";
-      "To" ::= "To";
+      "Type" ::= "$Type";
+      "To" ::= "$To";
       "From" ::= zero_val uint64T;
       "Term" ::= zero_val uint64T;
       "LogTerm" ::= zero_val uint64T;
@@ -352,7 +352,7 @@ Definition raft__maybeSendSnapshot : val :=
       "Entries" ::= zero_val sliceT;
       "Commit" ::= zero_val uint64T;
       "Vote" ::= zero_val uint64T;
-      "Snapshot" ::= "Snapshot";
+      "Snapshot" ::= "$Snapshot";
       "Reject" ::= zero_val boolT;
       "RejectHint" ::= zero_val uint64T;
       "Context" ::= zero_val sliceT;
@@ -814,21 +814,21 @@ Definition raft__maybeSendAppend : val :=
        let: "$a1" := (![ptrT] "pr") in
        (raft__maybeSendSnapshot (![ptrT] "r")) "$a0" "$a1")
     else do:  #());;;
-    do:  (let: "$a0" := (let: "To" := (![uint64T] "to") in
-    let: "Type" := raftpb.MsgApp in
-    let: "Index" := (![uint64T] "prevIndex") in
-    let: "LogTerm" := (![uint64T] "prevTerm") in
-    let: "Entries" := (![sliceT] "ents") in
-    let: "Commit" := (![uint64T] (struct.field_ref raftLog "committed" (![ptrT] (struct.field_ref raft "raftLog" (![ptrT] "r"))))) in
+    do:  (let: "$a0" := (let: "$To" := (![uint64T] "to") in
+    let: "$Type" := raftpb.MsgApp in
+    let: "$Index" := (![uint64T] "prevIndex") in
+    let: "$LogTerm" := (![uint64T] "prevTerm") in
+    let: "$Entries" := (![sliceT] "ents") in
+    let: "$Commit" := (![uint64T] (struct.field_ref raftLog "committed" (![ptrT] (struct.field_ref raft "raftLog" (![ptrT] "r"))))) in
     struct.make raftpb.Message [{
-      "Type" ::= "Type";
-      "To" ::= "To";
+      "Type" ::= "$Type";
+      "To" ::= "$To";
       "From" ::= zero_val uint64T;
       "Term" ::= zero_val uint64T;
-      "LogTerm" ::= "LogTerm";
-      "Index" ::= "Index";
-      "Entries" ::= "Entries";
-      "Commit" ::= "Commit";
+      "LogTerm" ::= "$LogTerm";
+      "Index" ::= "$Index";
+      "Entries" ::= "$Entries";
+      "Commit" ::= "$Commit";
       "Vote" ::= zero_val uint64T;
       "Snapshot" ::= zero_val ptrT;
       "Reject" ::= zero_val boolT;
@@ -923,11 +923,11 @@ Definition raft__maybeCommit : val :=
       "$f" "a0";;
       "$oldf" #()
       )));;;
-    return: (let: "$a0" := (let: "term" := (![uint64T] (struct.field_ref raft "Term" (![ptrT] "r"))) in
-     let: "index" := ((tracker.ProgressTracker__Committed (struct.field_ref raft "trk" (![ptrT] "r"))) #()) in
+    return: (let: "$a0" := (let: "$term" := (![uint64T] (struct.field_ref raft "Term" (![ptrT] "r"))) in
+     let: "$index" := ((tracker.ProgressTracker__Committed (struct.field_ref raft "trk" (![ptrT] "r"))) #()) in
      struct.make entryID [{
-       "term" ::= "term";
-       "index" ::= "index"
+       "term" ::= "$term";
+       "index" ::= "$index"
      }]) in
      (raftLog__maybeCommit (![ptrT] (struct.field_ref raft "raftLog" (![ptrT] "r")))) "$a0")).
 
@@ -985,11 +985,11 @@ Definition readOnly : go_type := structT [
 Definition newReadOnly : val :=
   rec: "newReadOnly" "option" :=
     exception_do (let: "option" := (ref_ty ReadOnlyOption "option") in
-    return: (ref_ty readOnly (let: "option" := (![ReadOnlyOption] "option") in
-     let: "pendingReadIndex" := (map.make stringT ptrT #()) in
+    return: (ref_ty readOnly (let: "$option" := (![ReadOnlyOption] "option") in
+     let: "$pendingReadIndex" := (map.make stringT ptrT #()) in
      struct.make readOnly [{
-       "option" ::= "option";
-       "pendingReadIndex" ::= "pendingReadIndex";
+       "option" ::= "$option";
+       "pendingReadIndex" ::= "$pendingReadIndex";
        "readIndexQueue" ::= zero_val sliceT
      }]))).
 
@@ -1047,22 +1047,22 @@ Definition raft__reset : val :=
     do:  (let: "$a0" := (λ: "id" "pr",
       exception_do (let: "pr" := (ref_ty ptrT "pr") in
       let: "id" := (ref_ty uint64T "id") in
-      let: "$r0" := (let: "Match" := #(W64 0) in
-      let: "Next" := (((raftLog__lastIndex (![ptrT] (struct.field_ref raft "raftLog" (![ptrT] "r")))) #()) + #(W64 1)) in
-      let: "Inflights" := (let: "$a0" := (![intT] (struct.field_ref tracker.ProgressTracker "MaxInflight" (struct.field_ref raft "trk" (![ptrT] "r")))) in
+      let: "$r0" := (let: "$Match" := #(W64 0) in
+      let: "$Next" := (((raftLog__lastIndex (![ptrT] (struct.field_ref raft "raftLog" (![ptrT] "r")))) #()) + #(W64 1)) in
+      let: "$Inflights" := (let: "$a0" := (![intT] (struct.field_ref tracker.ProgressTracker "MaxInflight" (struct.field_ref raft "trk" (![ptrT] "r")))) in
       let: "$a1" := (![uint64T] (struct.field_ref tracker.ProgressTracker "MaxInflightBytes" (struct.field_ref raft "trk" (![ptrT] "r")))) in
       tracker.NewInflights "$a0" "$a1") in
-      let: "IsLearner" := (![boolT] (struct.field_ref tracker.Progress "IsLearner" (![ptrT] "pr"))) in
+      let: "$IsLearner" := (![boolT] (struct.field_ref tracker.Progress "IsLearner" (![ptrT] "pr"))) in
       struct.make tracker.Progress [{
-        "Match" ::= "Match";
-        "Next" ::= "Next";
+        "Match" ::= "$Match";
+        "Next" ::= "$Next";
         "sentCommit" ::= zero_val uint64T;
         "State" ::= zero_val tracker.StateType;
         "PendingSnapshot" ::= zero_val uint64T;
         "RecentActive" ::= zero_val boolT;
         "MsgAppFlowPaused" ::= zero_val boolT;
-        "Inflights" ::= "Inflights";
-        "IsLearner" ::= "IsLearner"
+        "Inflights" ::= "$Inflights";
+        "IsLearner" ::= "$IsLearner"
       }]) in
       do:  ((![ptrT] "pr") <-[tracker.Progress] "$r0");;;
       (if: (![uint64T] "id") = (![uint64T] (struct.field_ref raft "id" (![ptrT] "r")))
@@ -1197,11 +1197,11 @@ Definition raft__applyConfChange : val :=
     let: "cfg" := (ref_ty tracker.Config (zero_val tracker.Config)) in
     let: (("$ret0", "$ret1"), "$ret2") := ((λ: <>,
       exception_do (let: "changer" := (ref_ty confchange.Changer (zero_val confchange.Changer)) in
-      let: "$r0" := (let: "Tracker" := (![tracker.ProgressTracker] (struct.field_ref raft "trk" (![ptrT] "r"))) in
-      let: "LastIndex" := ((raftLog__lastIndex (![ptrT] (struct.field_ref raft "raftLog" (![ptrT] "r")))) #()) in
+      let: "$r0" := (let: "$Tracker" := (![tracker.ProgressTracker] (struct.field_ref raft "trk" (![ptrT] "r"))) in
+      let: "$LastIndex" := ((raftLog__lastIndex (![ptrT] (struct.field_ref raft "raftLog" (![ptrT] "r")))) #()) in
       struct.make confchange.Changer [{
-        "Tracker" ::= "Tracker";
-        "LastIndex" ::= "LastIndex"
+        "Tracker" ::= "$Tracker";
+        "LastIndex" ::= "$LastIndex"
       }]) in
       do:  ("changer" <-[confchange.Changer] "$r0");;;
       (if: (raftpb.ConfChangeV2__LeaveJoint (![raftpb.ConfChangeV2] "cc")) #()
@@ -1362,13 +1362,13 @@ Definition RawNode__Bootstrap : val :=
       let: "i" := ref_ty uint64T "i" in
       let: "peer" := ref_ty Peer "peer" in
       let: "cc" := (ref_ty raftpb.ConfChange (zero_val raftpb.ConfChange)) in
-      let: "$r0" := (let: "Type" := raftpb.ConfChangeAddNode in
-      let: "NodeID" := (![uint64T] (struct.field_ref Peer "ID" "peer")) in
-      let: "Context" := (![sliceT] (struct.field_ref Peer "Context" "peer")) in
+      let: "$r0" := (let: "$Type" := raftpb.ConfChangeAddNode in
+      let: "$NodeID" := (![uint64T] (struct.field_ref Peer "ID" "peer")) in
+      let: "$Context" := (![sliceT] (struct.field_ref Peer "Context" "peer")) in
       struct.make raftpb.ConfChange [{
-        "Type" ::= "Type";
-        "NodeID" ::= "NodeID";
-        "Context" ::= "Context";
+        "Type" ::= "$Type";
+        "NodeID" ::= "$NodeID";
+        "Context" ::= "$Context";
         "ID" ::= zero_val uint64T
       }]) in
       do:  ("cc" <-[raftpb.ConfChange] "$r0");;;
@@ -1382,15 +1382,15 @@ Definition RawNode__Bootstrap : val :=
       (if: (![error] "err") ≠ #interface.nil
       then return: (![error] "err")
       else do:  #());;;
-      let: "$r0" := (let: "Type" := raftpb.EntryConfChange in
-      let: "Term" := #(W64 1) in
-      let: "Index" := ((![intT] "i") + #(W64 1)) in
-      let: "Data" := (![sliceT] "data") in
+      let: "$r0" := (let: "$Type" := raftpb.EntryConfChange in
+      let: "$Term" := #(W64 1) in
+      let: "$Index" := ((![intT] "i") + #(W64 1)) in
+      let: "$Data" := (![sliceT] "data") in
       struct.make raftpb.Entry [{
-        "Term" ::= "Term";
-        "Index" ::= "Index";
-        "Type" ::= "Type";
-        "Data" ::= "Data"
+        "Term" ::= "$Term";
+        "Index" ::= "$Index";
+        "Type" ::= "$Type";
+        "Data" ::= "$Data"
       }]) in
       do:  ((slice.elem_ref raftpb.Entry (![sliceT] "ents") (![intT] "i")) <-[raftpb.Entry] "$r0")));;;
     do:  (let: "$a0" := (![sliceT] "ents") in
@@ -1401,11 +1401,11 @@ Definition RawNode__Bootstrap : val :=
     do:  (let: "$range" := (![sliceT] "peers") in
     slice.for_range Peer "$range" (λ: <> "peer",
       let: "peer" := ref_ty Peer "peer" in
-      do:  (let: "$a0" := ((raftpb.ConfChange__AsV2 (let: "NodeID" := (![uint64T] (struct.field_ref Peer "ID" "peer")) in
-      let: "Type" := raftpb.ConfChangeAddNode in
+      do:  (let: "$a0" := ((raftpb.ConfChange__AsV2 (let: "$NodeID" := (![uint64T] (struct.field_ref Peer "ID" "peer")) in
+      let: "$Type" := raftpb.ConfChangeAddNode in
       struct.make raftpb.ConfChange [{
-        "Type" ::= "Type";
-        "NodeID" ::= "NodeID";
+        "Type" ::= "$Type";
+        "NodeID" ::= "$NodeID";
         "Context" ::= zero_val sliceT;
         "ID" ::= zero_val uint64T
       }])) #()) in
@@ -1588,11 +1588,11 @@ Definition raftLog__zeroTermOnOutOfBounds : val :=
 Definition pbEntryID : val :=
   rec: "pbEntryID" "entry" :=
     exception_do (let: "entry" := (ref_ty ptrT "entry") in
-    return: (let: "term" := (![uint64T] (struct.field_ref raftpb.Entry "Term" (![ptrT] "entry"))) in
-     let: "index" := (![uint64T] (struct.field_ref raftpb.Entry "Index" (![ptrT] "entry"))) in
+    return: (let: "$term" := (![uint64T] (struct.field_ref raftpb.Entry "Term" (![ptrT] "entry"))) in
+     let: "$index" := (![uint64T] (struct.field_ref raftpb.Entry "Index" (![ptrT] "entry"))) in
      struct.make entryID [{
-       "term" ::= "term";
-       "index" ::= "index"
+       "term" ::= "$term";
+       "index" ::= "$index"
      }])).
 
 (* findConflict finds the index of the conflict.
@@ -1800,11 +1800,11 @@ Definition raftLog__lastEntryID : val :=
       slice.literal interfaceT ["$sl0"; "$sl1"])) in
       (interface.get "Panicf" (![Logger] (struct.field_ref raftLog "logger" (![ptrT] "l")))) "$a0" "$a1")
     else do:  #());;;
-    return: (let: "term" := (![uint64T] "t") in
-     let: "index" := (![uint64T] "index") in
+    return: (let: "$term" := (![uint64T] "t") in
+     let: "$index" := (![uint64T] "index") in
      struct.make entryID [{
-       "term" ::= "term";
-       "index" ::= "index"
+       "term" ::= "$term";
+       "index" ::= "$index"
      }])).
 
 (* isUpToDate determines if a log with the given last entry is more up-to-date
@@ -2222,31 +2222,31 @@ Definition newLogWithSize : val :=
       do:  (let: "$a0" := (![error] "err") in
       Panic "$a0")
     else do:  #());;;
-    return: (ref_ty raftLog (let: "storage" := (![Storage] "storage") in
-     let: "unstable" := (let: "offset" := ((![uint64T] "lastIndex") + #(W64 1)) in
-     let: "offsetInProgress" := ((![uint64T] "lastIndex") + #(W64 1)) in
-     let: "logger" := (![Logger] "logger") in
+    return: (ref_ty raftLog (let: "$storage" := (![Storage] "storage") in
+     let: "$unstable" := (let: "$offset" := ((![uint64T] "lastIndex") + #(W64 1)) in
+     let: "$offsetInProgress" := ((![uint64T] "lastIndex") + #(W64 1)) in
+     let: "$logger" := (![Logger] "logger") in
      struct.make unstable [{
        "snapshot" ::= zero_val ptrT;
        "entries" ::= zero_val sliceT;
-       "offset" ::= "offset";
+       "offset" ::= "$offset";
        "snapshotInProgress" ::= zero_val boolT;
-       "offsetInProgress" ::= "offsetInProgress";
-       "logger" ::= "logger"
+       "offsetInProgress" ::= "$offsetInProgress";
+       "logger" ::= "$logger"
      }]) in
-     let: "maxApplyingEntsSize" := (![entryEncodingSize] "maxApplyingEntsSize") in
-     let: "committed" := ((![uint64T] "firstIndex") - #(W64 1)) in
-     let: "applying" := ((![uint64T] "firstIndex") - #(W64 1)) in
-     let: "applied" := ((![uint64T] "firstIndex") - #(W64 1)) in
-     let: "logger" := (![Logger] "logger") in
+     let: "$maxApplyingEntsSize" := (![entryEncodingSize] "maxApplyingEntsSize") in
+     let: "$committed" := ((![uint64T] "firstIndex") - #(W64 1)) in
+     let: "$applying" := ((![uint64T] "firstIndex") - #(W64 1)) in
+     let: "$applied" := ((![uint64T] "firstIndex") - #(W64 1)) in
+     let: "$logger" := (![Logger] "logger") in
      struct.make raftLog [{
-       "storage" ::= "storage";
-       "unstable" ::= "unstable";
-       "committed" ::= "committed";
-       "applying" ::= "applying";
-       "applied" ::= "applied";
-       "logger" ::= "logger";
-       "maxApplyingEntsSize" ::= "maxApplyingEntsSize";
+       "storage" ::= "$storage";
+       "unstable" ::= "$unstable";
+       "committed" ::= "$committed";
+       "applying" ::= "$applying";
+       "applied" ::= "$applied";
+       "logger" ::= "$logger";
+       "maxApplyingEntsSize" ::= "$maxApplyingEntsSize";
        "applyingEntsSize" ::= zero_val entryEncodingSize;
        "applyingEntsPaused" ::= zero_val boolT
      }]))).
@@ -2749,33 +2749,33 @@ Definition node : go_type := structT [
 Definition newNode : val :=
   rec: "newNode" "rn" :=
     exception_do (let: "rn" := (ref_ty ptrT "rn") in
-    return: (let: "propc" := (chan.make msgWithResult #()) in
-     let: "recvc" := (chan.make raftpb.Message #()) in
-     let: "confc" := (chan.make raftpb.ConfChangeV2 #()) in
-     let: "confstatec" := (chan.make raftpb.ConfState #()) in
-     let: "readyc" := (chan.make Ready #()) in
-     let: "advancec" := (chan.make (structT [
+    return: (let: "$propc" := (chan.make msgWithResult #()) in
+     let: "$recvc" := (chan.make raftpb.Message #()) in
+     let: "$confc" := (chan.make raftpb.ConfChangeV2 #()) in
+     let: "$confstatec" := (chan.make raftpb.ConfState #()) in
+     let: "$readyc" := (chan.make Ready #()) in
+     let: "$advancec" := (chan.make (structT [
      ]) #()) in
-     let: "tickc" := (chan.make (structT [
+     let: "$tickc" := (chan.make (structT [
      ]) #()) in
-     let: "done" := (chan.make (structT [
+     let: "$done" := (chan.make (structT [
      ]) #()) in
-     let: "stop" := (chan.make (structT [
+     let: "$stop" := (chan.make (structT [
      ]) #()) in
-     let: "status" := (chan.make (chanT Status) #()) in
-     let: "rn" := (![ptrT] "rn") in
+     let: "$status" := (chan.make (chanT Status) #()) in
+     let: "$rn" := (![ptrT] "rn") in
      struct.make node [{
-       "propc" ::= "propc";
-       "recvc" ::= "recvc";
-       "confc" ::= "confc";
-       "confstatec" ::= "confstatec";
-       "readyc" ::= "readyc";
-       "advancec" ::= "advancec";
-       "tickc" ::= "tickc";
-       "done" ::= "done";
-       "stop" ::= "stop";
-       "status" ::= "status";
-       "rn" ::= "rn"
+       "propc" ::= "$propc";
+       "recvc" ::= "$recvc";
+       "confc" ::= "$confc";
+       "confstatec" ::= "$confstatec";
+       "readyc" ::= "$readyc";
+       "advancec" ::= "$advancec";
+       "tickc" ::= "$tickc";
+       "done" ::= "$done";
+       "stop" ::= "$stop";
+       "status" ::= "$status";
+       "rn" ::= "$rn"
      }])).
 
 Definition Config : go_type := structT [
@@ -2804,24 +2804,24 @@ Definition Config : go_type := structT [
 Definition raft__hardState : val :=
   rec: "raft__hardState" "r" <> :=
     exception_do (let: "r" := (ref_ty ptrT "r") in
-    return: (let: "Term" := (![uint64T] (struct.field_ref raft "Term" (![ptrT] "r"))) in
-     let: "Vote" := (![uint64T] (struct.field_ref raft "Vote" (![ptrT] "r"))) in
-     let: "Commit" := (![uint64T] (struct.field_ref raftLog "committed" (![ptrT] (struct.field_ref raft "raftLog" (![ptrT] "r"))))) in
+    return: (let: "$Term" := (![uint64T] (struct.field_ref raft "Term" (![ptrT] "r"))) in
+     let: "$Vote" := (![uint64T] (struct.field_ref raft "Vote" (![ptrT] "r"))) in
+     let: "$Commit" := (![uint64T] (struct.field_ref raftLog "committed" (![ptrT] (struct.field_ref raft "raftLog" (![ptrT] "r"))))) in
      struct.make raftpb.HardState [{
-       "Term" ::= "Term";
-       "Vote" ::= "Vote";
-       "Commit" ::= "Commit"
+       "Term" ::= "$Term";
+       "Vote" ::= "$Vote";
+       "Commit" ::= "$Commit"
      }])).
 
 (* go: raft.go:508:16 *)
 Definition raft__softState : val :=
   rec: "raft__softState" "r" <> :=
     exception_do (let: "r" := (ref_ty ptrT "r") in
-    return: (let: "Lead" := (![uint64T] (struct.field_ref raft "lead" (![ptrT] "r"))) in
-     let: "RaftState" := (![StateType] (struct.field_ref raft "state" (![ptrT] "r"))) in
+    return: (let: "$Lead" := (![uint64T] (struct.field_ref raft "lead" (![ptrT] "r"))) in
+     let: "$RaftState" := (![StateType] (struct.field_ref raft "state" (![ptrT] "r"))) in
      struct.make SoftState [{
-       "Lead" ::= "Lead";
-       "RaftState" ::= "RaftState"
+       "Lead" ::= "$Lead";
+       "RaftState" ::= "$RaftState"
      }])).
 
 (* go: raft.go:2058:16 *)
@@ -2936,24 +2936,24 @@ Definition confChangeToMsg : val :=
          "Responses" ::= zero_val sliceT
        }], ![error] "err")
     else do:  #());;;
-    return: (let: "Type" := raftpb.MsgProp in
-     let: "Entries" := ((let: "$sl0" := (let: "Type" := (![raftpb.EntryType] "typ") in
-     let: "Data" := (![sliceT] "data") in
+    return: (let: "$Type" := raftpb.MsgProp in
+     let: "$Entries" := ((let: "$sl0" := (let: "$Type" := (![raftpb.EntryType] "typ") in
+     let: "$Data" := (![sliceT] "data") in
      struct.make raftpb.Entry [{
        "Term" ::= zero_val uint64T;
        "Index" ::= zero_val uint64T;
-       "Type" ::= "Type";
-       "Data" ::= "Data"
+       "Type" ::= "$Type";
+       "Data" ::= "$Data"
      }]) in
      slice.literal raftpb.Entry ["$sl0"])) in
      struct.make raftpb.Message [{
-       "Type" ::= "Type";
+       "Type" ::= "$Type";
        "To" ::= zero_val uint64T;
        "From" ::= zero_val uint64T;
        "Term" ::= zero_val uint64T;
        "LogTerm" ::= zero_val uint64T;
        "Index" ::= zero_val uint64T;
-       "Entries" ::= "Entries";
+       "Entries" ::= "$Entries";
        "Commit" ::= zero_val uint64T;
        "Vote" ::= zero_val uint64T;
        "Snapshot" ::= zero_val ptrT;
@@ -3166,15 +3166,15 @@ Definition raft__campaign : val :=
       let: "id" := ref_ty uint64T "id" in
       (if: (![uint64T] "id") = (![uint64T] (struct.field_ref raft "id" (![ptrT] "r")))
       then
-        do:  (let: "$a0" := (let: "To" := (![uint64T] "id") in
-        let: "Term" := (![uint64T] "term") in
-        let: "Type" := (let: "$a0" := (![raftpb.MessageType] "voteMsg") in
+        do:  (let: "$a0" := (let: "$To" := (![uint64T] "id") in
+        let: "$Term" := (![uint64T] "term") in
+        let: "$Type" := (let: "$a0" := (![raftpb.MessageType] "voteMsg") in
         voteRespMsgType "$a0") in
         struct.make raftpb.Message [{
-          "Type" ::= "Type";
-          "To" ::= "To";
+          "Type" ::= "$Type";
+          "To" ::= "$To";
           "From" ::= zero_val uint64T;
-          "Term" ::= "Term";
+          "Term" ::= "$Term";
           "LogTerm" ::= zero_val uint64T;
           "Index" ::= zero_val uint64T;
           "Entries" ::= zero_val sliceT;
@@ -3207,26 +3207,26 @@ Definition raft__campaign : val :=
         let: "$r0" := (string.to_bytes (![CampaignType] "t")) in
         do:  ("ctx" <-[sliceT] "$r0")
       else do:  #());;;
-      do:  (let: "$a0" := (let: "To" := (![uint64T] "id") in
-      let: "Term" := (![uint64T] "term") in
-      let: "Type" := (![raftpb.MessageType] "voteMsg") in
-      let: "Index" := (![uint64T] (struct.field_ref entryID "index" "last")) in
-      let: "LogTerm" := (![uint64T] (struct.field_ref entryID "term" "last")) in
-      let: "Context" := (![sliceT] "ctx") in
+      do:  (let: "$a0" := (let: "$To" := (![uint64T] "id") in
+      let: "$Term" := (![uint64T] "term") in
+      let: "$Type" := (![raftpb.MessageType] "voteMsg") in
+      let: "$Index" := (![uint64T] (struct.field_ref entryID "index" "last")) in
+      let: "$LogTerm" := (![uint64T] (struct.field_ref entryID "term" "last")) in
+      let: "$Context" := (![sliceT] "ctx") in
       struct.make raftpb.Message [{
-        "Type" ::= "Type";
-        "To" ::= "To";
+        "Type" ::= "$Type";
+        "To" ::= "$To";
         "From" ::= zero_val uint64T;
-        "Term" ::= "Term";
-        "LogTerm" ::= "LogTerm";
-        "Index" ::= "Index";
+        "Term" ::= "$Term";
+        "LogTerm" ::= "$LogTerm";
+        "Index" ::= "$Index";
         "Entries" ::= zero_val sliceT;
         "Commit" ::= zero_val uint64T;
         "Vote" ::= zero_val uint64T;
         "Snapshot" ::= zero_val ptrT;
         "Reject" ::= zero_val boolT;
         "RejectHint" ::= zero_val uint64T;
-        "Context" ::= "Context";
+        "Context" ::= "$Context";
         "Responses" ::= zero_val sliceT
       }]) in
       (raft__send (![ptrT] "r")) "$a0")))).
@@ -3401,11 +3401,11 @@ Definition raft__Step : val :=
         then
           (if: ((![boolT] (struct.field_ref raft "checkQuorum" (![ptrT] "r"))) || (![boolT] (struct.field_ref raft "preVote" (![ptrT] "r")))) && (((![raftpb.MessageType] (struct.field_ref raftpb.Message "Type" "m")) = raftpb.MsgHeartbeat) || ((![raftpb.MessageType] (struct.field_ref raftpb.Message "Type" "m")) = raftpb.MsgApp))
           then
-            do:  (let: "$a0" := (let: "To" := (![uint64T] (struct.field_ref raftpb.Message "From" "m")) in
-            let: "Type" := raftpb.MsgAppResp in
+            do:  (let: "$a0" := (let: "$To" := (![uint64T] (struct.field_ref raftpb.Message "From" "m")) in
+            let: "$Type" := raftpb.MsgAppResp in
             struct.make raftpb.Message [{
-              "Type" ::= "Type";
-              "To" ::= "To";
+              "Type" ::= "$Type";
+              "To" ::= "$To";
               "From" ::= zero_val uint64T;
               "Term" ::= zero_val uint64T;
               "LogTerm" ::= zero_val uint64T;
@@ -3438,22 +3438,22 @@ Definition raft__Step : val :=
               let: "$sl8" := (interface.make uint64__mset (![uint64T] (struct.field_ref raft "Term" (![ptrT] "r")))) in
               slice.literal interfaceT ["$sl0"; "$sl1"; "$sl2"; "$sl3"; "$sl4"; "$sl5"; "$sl6"; "$sl7"; "$sl8"])) in
               (interface.get "Infof" (![Logger] (struct.field_ref raft "logger" (![ptrT] "r")))) "$a0" "$a1");;;
-              do:  (let: "$a0" := (let: "To" := (![uint64T] (struct.field_ref raftpb.Message "From" "m")) in
-              let: "Term" := (![uint64T] (struct.field_ref raft "Term" (![ptrT] "r"))) in
-              let: "Type" := raftpb.MsgPreVoteResp in
-              let: "Reject" := #true in
+              do:  (let: "$a0" := (let: "$To" := (![uint64T] (struct.field_ref raftpb.Message "From" "m")) in
+              let: "$Term" := (![uint64T] (struct.field_ref raft "Term" (![ptrT] "r"))) in
+              let: "$Type" := raftpb.MsgPreVoteResp in
+              let: "$Reject" := #true in
               struct.make raftpb.Message [{
-                "Type" ::= "Type";
-                "To" ::= "To";
+                "Type" ::= "$Type";
+                "To" ::= "$To";
                 "From" ::= zero_val uint64T;
-                "Term" ::= "Term";
+                "Term" ::= "$Term";
                 "LogTerm" ::= zero_val uint64T;
                 "Index" ::= zero_val uint64T;
                 "Entries" ::= zero_val sliceT;
                 "Commit" ::= zero_val uint64T;
                 "Vote" ::= zero_val uint64T;
                 "Snapshot" ::= zero_val ptrT;
-                "Reject" ::= "Reject";
+                "Reject" ::= "$Reject";
                 "RejectHint" ::= zero_val uint64T;
                 "Context" ::= zero_val sliceT;
                 "Responses" ::= zero_val sliceT
@@ -3503,11 +3503,11 @@ Definition raft__Step : val :=
       then
         (if: (![uint64T] (struct.field_ref raftpb.Message "Index" "m")) ≠ #(W64 0)
         then
-          do:  (let: "$a0" := (let: "term" := (![uint64T] (struct.field_ref raftpb.Message "LogTerm" "m")) in
-          let: "index" := (![uint64T] (struct.field_ref raftpb.Message "Index" "m")) in
+          do:  (let: "$a0" := (let: "$term" := (![uint64T] (struct.field_ref raftpb.Message "LogTerm" "m")) in
+          let: "$index" := (![uint64T] (struct.field_ref raftpb.Message "Index" "m")) in
           struct.make entryID [{
-            "term" ::= "term";
-            "index" ::= "index"
+            "term" ::= "$term";
+            "index" ::= "$index"
           }]) in
           (raftLog__stableTo (![ptrT] (struct.field_ref raft "raftLog" (![ptrT] "r")))) "$a0")
         else do:  #());;;
@@ -3544,11 +3544,11 @@ Definition raft__Step : val :=
             let: "$r0" := ((raftLog__lastEntryID (![ptrT] (struct.field_ref raft "raftLog" (![ptrT] "r")))) #()) in
             do:  ("lastID" <-[entryID] "$r0");;;
             let: "candLastID" := (ref_ty entryID (zero_val entryID)) in
-            let: "$r0" := (let: "term" := (![uint64T] (struct.field_ref raftpb.Message "LogTerm" "m")) in
-            let: "index" := (![uint64T] (struct.field_ref raftpb.Message "Index" "m")) in
+            let: "$r0" := (let: "$term" := (![uint64T] (struct.field_ref raftpb.Message "LogTerm" "m")) in
+            let: "$index" := (![uint64T] (struct.field_ref raftpb.Message "Index" "m")) in
             struct.make entryID [{
-              "term" ::= "term";
-              "index" ::= "index"
+              "term" ::= "$term";
+              "index" ::= "$index"
             }]) in
             do:  ("candLastID" <-[entryID] "$r0");;;
             (if: (![boolT] "canVote") && (let: "$a0" := (![entryID] "candLastID") in
@@ -3566,15 +3566,15 @@ Definition raft__Step : val :=
               let: "$sl8" := (interface.make uint64__mset (![uint64T] (struct.field_ref raft "Term" (![ptrT] "r")))) in
               slice.literal interfaceT ["$sl0"; "$sl1"; "$sl2"; "$sl3"; "$sl4"; "$sl5"; "$sl6"; "$sl7"; "$sl8"])) in
               (interface.get "Infof" (![Logger] (struct.field_ref raft "logger" (![ptrT] "r")))) "$a0" "$a1");;;
-              do:  (let: "$a0" := (let: "To" := (![uint64T] (struct.field_ref raftpb.Message "From" "m")) in
-              let: "Term" := (![uint64T] (struct.field_ref raftpb.Message "Term" "m")) in
-              let: "Type" := (let: "$a0" := (![raftpb.MessageType] (struct.field_ref raftpb.Message "Type" "m")) in
+              do:  (let: "$a0" := (let: "$To" := (![uint64T] (struct.field_ref raftpb.Message "From" "m")) in
+              let: "$Term" := (![uint64T] (struct.field_ref raftpb.Message "Term" "m")) in
+              let: "$Type" := (let: "$a0" := (![raftpb.MessageType] (struct.field_ref raftpb.Message "Type" "m")) in
               voteRespMsgType "$a0") in
               struct.make raftpb.Message [{
-                "Type" ::= "Type";
-                "To" ::= "To";
+                "Type" ::= "$Type";
+                "To" ::= "$To";
                 "From" ::= zero_val uint64T;
-                "Term" ::= "Term";
+                "Term" ::= "$Term";
                 "LogTerm" ::= zero_val uint64T;
                 "Index" ::= zero_val uint64T;
                 "Entries" ::= zero_val sliceT;
@@ -3607,23 +3607,23 @@ Definition raft__Step : val :=
               let: "$sl8" := (interface.make uint64__mset (![uint64T] (struct.field_ref raft "Term" (![ptrT] "r")))) in
               slice.literal interfaceT ["$sl0"; "$sl1"; "$sl2"; "$sl3"; "$sl4"; "$sl5"; "$sl6"; "$sl7"; "$sl8"])) in
               (interface.get "Infof" (![Logger] (struct.field_ref raft "logger" (![ptrT] "r")))) "$a0" "$a1");;;
-              do:  (let: "$a0" := (let: "To" := (![uint64T] (struct.field_ref raftpb.Message "From" "m")) in
-              let: "Term" := (![uint64T] (struct.field_ref raft "Term" (![ptrT] "r"))) in
-              let: "Type" := (let: "$a0" := (![raftpb.MessageType] (struct.field_ref raftpb.Message "Type" "m")) in
+              do:  (let: "$a0" := (let: "$To" := (![uint64T] (struct.field_ref raftpb.Message "From" "m")) in
+              let: "$Term" := (![uint64T] (struct.field_ref raft "Term" (![ptrT] "r"))) in
+              let: "$Type" := (let: "$a0" := (![raftpb.MessageType] (struct.field_ref raftpb.Message "Type" "m")) in
               voteRespMsgType "$a0") in
-              let: "Reject" := #true in
+              let: "$Reject" := #true in
               struct.make raftpb.Message [{
-                "Type" ::= "Type";
-                "To" ::= "To";
+                "Type" ::= "$Type";
+                "To" ::= "$To";
                 "From" ::= zero_val uint64T;
-                "Term" ::= "Term";
+                "Term" ::= "$Term";
                 "LogTerm" ::= zero_val uint64T;
                 "Index" ::= zero_val uint64T;
                 "Entries" ::= zero_val sliceT;
                 "Commit" ::= zero_val uint64T;
                 "Vote" ::= zero_val uint64T;
                 "Snapshot" ::= zero_val ptrT;
-                "Reject" ::= "Reject";
+                "Reject" ::= "$Reject";
                 "RejectHint" ::= zero_val uint64T;
                 "Context" ::= zero_val sliceT;
                 "Responses" ::= zero_val sliceT
@@ -3753,60 +3753,60 @@ Definition newRaft : val :=
       Panic "$a0")
     else do:  #());;;
     let: "r" := (ref_ty ptrT (zero_val ptrT)) in
-    let: "$r0" := (ref_ty raft (let: "id" := (![uint64T] (struct.field_ref Config "ID" (![ptrT] "c"))) in
-    let: "lead" := None in
-    let: "isLearner" := #false in
-    let: "raftLog" := (![ptrT] "raftlog") in
-    let: "maxMsgSize" := (![uint64T] (struct.field_ref Config "MaxSizePerMsg" (![ptrT] "c"))) in
-    let: "maxUncommittedSize" := (![uint64T] (struct.field_ref Config "MaxUncommittedEntriesSize" (![ptrT] "c"))) in
-    let: "trk" := (let: "$a0" := (![intT] (struct.field_ref Config "MaxInflightMsgs" (![ptrT] "c"))) in
+    let: "$r0" := (ref_ty raft (let: "$id" := (![uint64T] (struct.field_ref Config "ID" (![ptrT] "c"))) in
+    let: "$lead" := None in
+    let: "$isLearner" := #false in
+    let: "$raftLog" := (![ptrT] "raftlog") in
+    let: "$maxMsgSize" := (![uint64T] (struct.field_ref Config "MaxSizePerMsg" (![ptrT] "c"))) in
+    let: "$maxUncommittedSize" := (![uint64T] (struct.field_ref Config "MaxUncommittedEntriesSize" (![ptrT] "c"))) in
+    let: "$trk" := (let: "$a0" := (![intT] (struct.field_ref Config "MaxInflightMsgs" (![ptrT] "c"))) in
     let: "$a1" := (![uint64T] (struct.field_ref Config "MaxInflightBytes" (![ptrT] "c"))) in
     tracker.MakeProgressTracker "$a0" "$a1") in
-    let: "electionTimeout" := (![intT] (struct.field_ref Config "ElectionTick" (![ptrT] "c"))) in
-    let: "heartbeatTimeout" := (![intT] (struct.field_ref Config "HeartbeatTick" (![ptrT] "c"))) in
-    let: "logger" := (![Logger] (struct.field_ref Config "Logger" (![ptrT] "c"))) in
-    let: "checkQuorum" := (![boolT] (struct.field_ref Config "CheckQuorum" (![ptrT] "c"))) in
-    let: "preVote" := (![boolT] (struct.field_ref Config "PreVote" (![ptrT] "c"))) in
-    let: "readOnly" := (let: "$a0" := (![ReadOnlyOption] (struct.field_ref Config "ReadOnlyOption" (![ptrT] "c"))) in
+    let: "$electionTimeout" := (![intT] (struct.field_ref Config "ElectionTick" (![ptrT] "c"))) in
+    let: "$heartbeatTimeout" := (![intT] (struct.field_ref Config "HeartbeatTick" (![ptrT] "c"))) in
+    let: "$logger" := (![Logger] (struct.field_ref Config "Logger" (![ptrT] "c"))) in
+    let: "$checkQuorum" := (![boolT] (struct.field_ref Config "CheckQuorum" (![ptrT] "c"))) in
+    let: "$preVote" := (![boolT] (struct.field_ref Config "PreVote" (![ptrT] "c"))) in
+    let: "$readOnly" := (let: "$a0" := (![ReadOnlyOption] (struct.field_ref Config "ReadOnlyOption" (![ptrT] "c"))) in
     newReadOnly "$a0") in
-    let: "disableProposalForwarding" := (![boolT] (struct.field_ref Config "DisableProposalForwarding" (![ptrT] "c"))) in
-    let: "disableConfChangeValidation" := (![boolT] (struct.field_ref Config "DisableConfChangeValidation" (![ptrT] "c"))) in
-    let: "stepDownOnRemoval" := (![boolT] (struct.field_ref Config "StepDownOnRemoval" (![ptrT] "c"))) in
-    let: "traceLogger" := (![TraceLogger] (struct.field_ref Config "TraceLogger" (![ptrT] "c"))) in
+    let: "$disableProposalForwarding" := (![boolT] (struct.field_ref Config "DisableProposalForwarding" (![ptrT] "c"))) in
+    let: "$disableConfChangeValidation" := (![boolT] (struct.field_ref Config "DisableConfChangeValidation" (![ptrT] "c"))) in
+    let: "$stepDownOnRemoval" := (![boolT] (struct.field_ref Config "StepDownOnRemoval" (![ptrT] "c"))) in
+    let: "$traceLogger" := (![TraceLogger] (struct.field_ref Config "TraceLogger" (![ptrT] "c"))) in
     struct.make raft [{
-      "id" ::= "id";
+      "id" ::= "$id";
       "Term" ::= zero_val uint64T;
       "Vote" ::= zero_val uint64T;
       "readStates" ::= zero_val sliceT;
-      "raftLog" ::= "raftLog";
-      "maxMsgSize" ::= "maxMsgSize";
-      "maxUncommittedSize" ::= "maxUncommittedSize";
-      "trk" ::= "trk";
+      "raftLog" ::= "$raftLog";
+      "maxMsgSize" ::= "$maxMsgSize";
+      "maxUncommittedSize" ::= "$maxUncommittedSize";
+      "trk" ::= "$trk";
       "state" ::= zero_val StateType;
-      "isLearner" ::= "isLearner";
+      "isLearner" ::= "$isLearner";
       "msgs" ::= zero_val sliceT;
       "msgsAfterAppend" ::= zero_val sliceT;
-      "lead" ::= "lead";
+      "lead" ::= "$lead";
       "leadTransferee" ::= zero_val uint64T;
       "pendingConfIndex" ::= zero_val uint64T;
-      "disableConfChangeValidation" ::= "disableConfChangeValidation";
+      "disableConfChangeValidation" ::= "$disableConfChangeValidation";
       "uncommittedSize" ::= zero_val entryPayloadSize;
-      "readOnly" ::= "readOnly";
+      "readOnly" ::= "$readOnly";
       "electionElapsed" ::= zero_val intT;
       "heartbeatElapsed" ::= zero_val intT;
-      "checkQuorum" ::= "checkQuorum";
-      "preVote" ::= "preVote";
-      "heartbeatTimeout" ::= "heartbeatTimeout";
-      "electionTimeout" ::= "electionTimeout";
+      "checkQuorum" ::= "$checkQuorum";
+      "preVote" ::= "$preVote";
+      "heartbeatTimeout" ::= "$heartbeatTimeout";
+      "electionTimeout" ::= "$electionTimeout";
       "randomizedElectionTimeout" ::= zero_val intT;
-      "disableProposalForwarding" ::= "disableProposalForwarding";
-      "stepDownOnRemoval" ::= "stepDownOnRemoval";
+      "disableProposalForwarding" ::= "$disableProposalForwarding";
+      "stepDownOnRemoval" ::= "$stepDownOnRemoval";
       "tickId" ::= zero_val intT;
       "step" ::= zero_val funcT;
       "StepHigherOrder" ::= zero_val funcT;
-      "logger" ::= "logger";
+      "logger" ::= "$logger";
       "pendingReadIndexMessages" ::= zero_val sliceT;
-      "traceLogger" ::= "traceLogger"
+      "traceLogger" ::= "$traceLogger"
     }])) in
     do:  ("r" <-[ptrT] "$r0");;;
     let: "$r0" := (raft__Step (![ptrT] "r")) in
@@ -3818,11 +3818,11 @@ Definition newRaft : val :=
     do:  ("lastID" <-[entryID] "$r0");;;
     let: "trk" := (ref_ty tracker.ProgressMap (zero_val tracker.ProgressMap)) in
     let: "cfg" := (ref_ty tracker.Config (zero_val tracker.Config)) in
-    let: (("$ret0", "$ret1"), "$ret2") := (let: "$a0" := (let: "Tracker" := (![tracker.ProgressTracker] (struct.field_ref raft "trk" (![ptrT] "r"))) in
-    let: "LastIndex" := (![uint64T] (struct.field_ref entryID "index" "lastID")) in
+    let: (("$ret0", "$ret1"), "$ret2") := (let: "$a0" := (let: "$Tracker" := (![tracker.ProgressTracker] (struct.field_ref raft "trk" (![ptrT] "r"))) in
+    let: "$LastIndex" := (![uint64T] (struct.field_ref entryID "index" "lastID")) in
     struct.make confchange.Changer [{
-      "Tracker" ::= "Tracker";
-      "LastIndex" ::= "LastIndex"
+      "Tracker" ::= "$Tracker";
+      "LastIndex" ::= "$LastIndex"
     }]) in
     let: "$a1" := (![raftpb.ConfState] "cs") in
     confchange.Restore "$a0" "$a1") in
@@ -3901,9 +3901,9 @@ Definition NewRawNode : val :=
     newRaft "$a0") in
     do:  ("r" <-[ptrT] "$r0");;;
     let: "rn" := (ref_ty ptrT (zero_val ptrT)) in
-    let: "$r0" := (ref_ty RawNode (let: "raft" := (![ptrT] "r") in
+    let: "$r0" := (ref_ty RawNode (let: "$raft" := (![ptrT] "r") in
     struct.make RawNode [{
-      "raft" ::= "raft";
+      "raft" ::= "$raft";
       "asyncStorageWrites" ::= zero_val boolT;
       "prevSoftSt" ::= zero_val ptrT;
       "prevHardSt" ::= zero_val raftpb.HardState;
@@ -4015,9 +4015,9 @@ Definition node__stepWithWaitOption : val :=
     let: "$r0" := (![chanT msgWithResult] (struct.field_ref node "propc" (![ptrT] "n"))) in
     do:  ("ch" <-[chanT msgWithResult] "$r0");;;
     let: "pm" := (ref_ty msgWithResult (zero_val msgWithResult)) in
-    let: "$r0" := (let: "m" := (![raftpb.Message] "m") in
+    let: "$r0" := (let: "$m" := (![raftpb.Message] "m") in
     struct.make msgWithResult [{
-      "m" ::= "m";
+      "m" ::= "$m";
       "result" ::= zero_val (chanT error)
     }]) in
     do:  ("pm" <-[msgWithResult] "$r0");;;
@@ -4066,9 +4066,9 @@ Definition node__Campaign : val :=
     exception_do (let: "n" := (ref_ty ptrT "n") in
     let: "ctx" := (ref_ty context.Context "ctx") in
     return: (let: "$a0" := (![context.Context] "ctx") in
-     let: "$a1" := (let: "Type" := raftpb.MsgHup in
+     let: "$a1" := (let: "$Type" := raftpb.MsgHup in
      struct.make raftpb.Message [{
-       "Type" ::= "Type";
+       "Type" ::= "$Type";
        "To" ::= zero_val uint64T;
        "From" ::= zero_val uint64T;
        "Term" ::= zero_val uint64T;
@@ -4091,9 +4091,9 @@ Definition node__ForgetLeader : val :=
     exception_do (let: "n" := (ref_ty ptrT "n") in
     let: "ctx" := (ref_ty context.Context "ctx") in
     return: (let: "$a0" := (![context.Context] "ctx") in
-     let: "$a1" := (let: "Type" := raftpb.MsgForgetLeader in
+     let: "$a1" := (let: "$Type" := raftpb.MsgForgetLeader in
      struct.make raftpb.Message [{
-       "Type" ::= "Type";
+       "Type" ::= "$Type";
        "To" ::= zero_val uint64T;
        "From" ::= zero_val uint64T;
        "Term" ::= zero_val uint64T;
@@ -4128,23 +4128,23 @@ Definition node__Propose : val :=
     let: "data" := (ref_ty sliceT "data") in
     let: "ctx" := (ref_ty context.Context "ctx") in
     return: (let: "$a0" := (![context.Context] "ctx") in
-     let: "$a1" := (let: "Type" := raftpb.MsgProp in
-     let: "Entries" := ((let: "$sl0" := (let: "Data" := (![sliceT] "data") in
+     let: "$a1" := (let: "$Type" := raftpb.MsgProp in
+     let: "$Entries" := ((let: "$sl0" := (let: "$Data" := (![sliceT] "data") in
      struct.make raftpb.Entry [{
        "Term" ::= zero_val uint64T;
        "Index" ::= zero_val uint64T;
        "Type" ::= zero_val raftpb.EntryType;
-       "Data" ::= "Data"
+       "Data" ::= "$Data"
      }]) in
      slice.literal raftpb.Entry ["$sl0"])) in
      struct.make raftpb.Message [{
-       "Type" ::= "Type";
+       "Type" ::= "$Type";
        "To" ::= zero_val uint64T;
        "From" ::= zero_val uint64T;
        "Term" ::= zero_val uint64T;
        "LogTerm" ::= zero_val uint64T;
        "Index" ::= zero_val uint64T;
-       "Entries" ::= "Entries";
+       "Entries" ::= "$Entries";
        "Commit" ::= zero_val uint64T;
        "Vote" ::= zero_val uint64T;
        "Snapshot" ::= zero_val ptrT;
@@ -4218,23 +4218,23 @@ Definition node__ReadIndex : val :=
     let: "rctx" := (ref_ty sliceT "rctx") in
     let: "ctx" := (ref_ty context.Context "ctx") in
     return: (let: "$a0" := (![context.Context] "ctx") in
-     let: "$a1" := (let: "Type" := raftpb.MsgReadIndex in
-     let: "Entries" := ((let: "$sl0" := (let: "Data" := (![sliceT] "rctx") in
+     let: "$a1" := (let: "$Type" := raftpb.MsgReadIndex in
+     let: "$Entries" := ((let: "$sl0" := (let: "$Data" := (![sliceT] "rctx") in
      struct.make raftpb.Entry [{
        "Term" ::= zero_val uint64T;
        "Index" ::= zero_val uint64T;
        "Type" ::= zero_val raftpb.EntryType;
-       "Data" ::= "Data"
+       "Data" ::= "$Data"
      }]) in
      slice.literal raftpb.Entry ["$sl0"])) in
      struct.make raftpb.Message [{
-       "Type" ::= "Type";
+       "Type" ::= "$Type";
        "To" ::= zero_val uint64T;
        "From" ::= zero_val uint64T;
        "Term" ::= zero_val uint64T;
        "LogTerm" ::= zero_val uint64T;
        "Index" ::= zero_val uint64T;
-       "Entries" ::= "Entries";
+       "Entries" ::= "$Entries";
        "Commit" ::= zero_val uint64T;
        "Vote" ::= zero_val uint64T;
        "Snapshot" ::= zero_val ptrT;
@@ -4365,12 +4365,12 @@ Definition raft__tickHeartbeat : val :=
       (if: ![boolT] (struct.field_ref raft "checkQuorum" (![ptrT] "r"))
       then
         (let: "err" := (ref_ty error (zero_val error)) in
-        let: "$r0" := (let: "$a0" := (let: "From" := (![uint64T] (struct.field_ref raft "id" (![ptrT] "r"))) in
-        let: "Type" := raftpb.MsgCheckQuorum in
+        let: "$r0" := (let: "$a0" := (let: "$From" := (![uint64T] (struct.field_ref raft "id" (![ptrT] "r"))) in
+        let: "$Type" := raftpb.MsgCheckQuorum in
         struct.make raftpb.Message [{
-          "Type" ::= "Type";
+          "Type" ::= "$Type";
           "To" ::= zero_val uint64T;
-          "From" ::= "From";
+          "From" ::= "$From";
           "Term" ::= zero_val uint64T;
           "LogTerm" ::= zero_val uint64T;
           "Index" ::= zero_val uint64T;
@@ -4405,12 +4405,12 @@ Definition raft__tickHeartbeat : val :=
       let: "$r0" := #(W64 0) in
       do:  ((struct.field_ref raft "heartbeatElapsed" (![ptrT] "r")) <-[intT] "$r0");;;
       (let: "err" := (ref_ty error (zero_val error)) in
-      let: "$r0" := (let: "$a0" := (let: "From" := (![uint64T] (struct.field_ref raft "id" (![ptrT] "r"))) in
-      let: "Type" := raftpb.MsgBeat in
+      let: "$r0" := (let: "$a0" := (let: "$From" := (![uint64T] (struct.field_ref raft "id" (![ptrT] "r"))) in
+      let: "$Type" := raftpb.MsgBeat in
       struct.make raftpb.Message [{
-        "Type" ::= "Type";
+        "Type" ::= "$Type";
         "To" ::= zero_val uint64T;
-        "From" ::= "From";
+        "From" ::= "$From";
         "Term" ::= zero_val uint64T;
         "LogTerm" ::= zero_val uint64T;
         "Index" ::= zero_val uint64T;
@@ -4456,12 +4456,12 @@ Definition raft__tickElection : val :=
       let: "$r0" := #(W64 0) in
       do:  ((struct.field_ref raft "electionElapsed" (![ptrT] "r")) <-[intT] "$r0");;;
       (let: "err" := (ref_ty error (zero_val error)) in
-      let: "$r0" := (let: "$a0" := (let: "From" := (![uint64T] (struct.field_ref raft "id" (![ptrT] "r"))) in
-      let: "Type" := raftpb.MsgHup in
+      let: "$r0" := (let: "$a0" := (let: "$From" := (![uint64T] (struct.field_ref raft "id" (![ptrT] "r"))) in
+      let: "$Type" := raftpb.MsgHup in
       struct.make raftpb.Message [{
-        "Type" ::= "Type";
+        "Type" ::= "$Type";
         "To" ::= zero_val uint64T;
-        "From" ::= "From";
+        "From" ::= "$From";
         "Term" ::= zero_val uint64T;
         "LogTerm" ::= zero_val uint64T;
         "Index" ::= zero_val uint64T;
@@ -4544,19 +4544,19 @@ Definition newStorageApplyRespMsg : val :=
   rec: "newStorageApplyRespMsg" "r" "ents" :=
     exception_do (let: "ents" := (ref_ty sliceT "ents") in
     let: "r" := (ref_ty ptrT "r") in
-    return: (let: "Type" := raftpb.MsgStorageApplyResp in
-     let: "To" := (![uint64T] (struct.field_ref raft "id" (![ptrT] "r"))) in
-     let: "From" := LocalApplyThread in
-     let: "Term" := #(W64 0) in
-     let: "Entries" := (![sliceT] "ents") in
+    return: (let: "$Type" := raftpb.MsgStorageApplyResp in
+     let: "$To" := (![uint64T] (struct.field_ref raft "id" (![ptrT] "r"))) in
+     let: "$From" := LocalApplyThread in
+     let: "$Term" := #(W64 0) in
+     let: "$Entries" := (![sliceT] "ents") in
      struct.make raftpb.Message [{
-       "Type" ::= "Type";
-       "To" ::= "To";
-       "From" ::= "From";
-       "Term" ::= "Term";
+       "Type" ::= "$Type";
+       "To" ::= "$To";
+       "From" ::= "$From";
+       "Term" ::= "$Term";
        "LogTerm" ::= zero_val uint64T;
        "Index" ::= zero_val uint64T;
-       "Entries" ::= "Entries";
+       "Entries" ::= "$Entries";
        "Commit" ::= zero_val uint64T;
        "Vote" ::= zero_val uint64T;
        "Snapshot" ::= zero_val ptrT;
@@ -4585,15 +4585,15 @@ Definition newStorageAppendRespMsg : val :=
     exception_do (let: "rd" := (ref_ty Ready "rd") in
     let: "r" := (ref_ty ptrT "r") in
     let: "m" := (ref_ty raftpb.Message (zero_val raftpb.Message)) in
-    let: "$r0" := (let: "Type" := raftpb.MsgStorageAppendResp in
-    let: "To" := (![uint64T] (struct.field_ref raft "id" (![ptrT] "r"))) in
-    let: "From" := LocalAppendThread in
-    let: "Term" := (![uint64T] (struct.field_ref raft "Term" (![ptrT] "r"))) in
+    let: "$r0" := (let: "$Type" := raftpb.MsgStorageAppendResp in
+    let: "$To" := (![uint64T] (struct.field_ref raft "id" (![ptrT] "r"))) in
+    let: "$From" := LocalAppendThread in
+    let: "$Term" := (![uint64T] (struct.field_ref raft "Term" (![ptrT] "r"))) in
     struct.make raftpb.Message [{
-      "Type" ::= "Type";
-      "To" ::= "To";
-      "From" ::= "From";
-      "Term" ::= "Term";
+      "Type" ::= "$Type";
+      "To" ::= "$To";
+      "From" ::= "$From";
+      "Term" ::= "$Term";
       "LogTerm" ::= zero_val uint64T;
       "Index" ::= zero_val uint64T;
       "Entries" ::= zero_val sliceT;
@@ -4800,14 +4800,14 @@ Definition getBasicStatus : val :=
   rec: "getBasicStatus" "r" :=
     exception_do (let: "r" := (ref_ty ptrT "r") in
     let: "s" := (ref_ty BasicStatus (zero_val BasicStatus)) in
-    let: "$r0" := (let: "ID" := (![uint64T] (struct.field_ref raft "id" (![ptrT] "r"))) in
-    let: "LeadTransferee" := (![uint64T] (struct.field_ref raft "leadTransferee" (![ptrT] "r"))) in
+    let: "$r0" := (let: "$ID" := (![uint64T] (struct.field_ref raft "id" (![ptrT] "r"))) in
+    let: "$LeadTransferee" := (![uint64T] (struct.field_ref raft "leadTransferee" (![ptrT] "r"))) in
     struct.make BasicStatus [{
-      "ID" ::= "ID";
+      "ID" ::= "$ID";
       "HardState" ::= zero_val raftpb.HardState;
       "SoftState" ::= zero_val SoftState;
       "Applied" ::= zero_val uint64T;
-      "LeadTransferee" ::= "LeadTransferee"
+      "LeadTransferee" ::= "$LeadTransferee"
     }]) in
     do:  ("s" <-[BasicStatus] "$r0");;;
     let: "$r0" := ((raft__hardState (![ptrT] "r")) #()) in
@@ -4900,30 +4900,30 @@ Definition newStorageApplyMsg : val :=
     let: "ents" := (ref_ty sliceT (zero_val sliceT)) in
     let: "$r0" := (![sliceT] (struct.field_ref Ready "CommittedEntries" "rd")) in
     do:  ("ents" <-[sliceT] "$r0");;;
-    return: (let: "Type" := raftpb.MsgStorageApply in
-     let: "To" := LocalApplyThread in
-     let: "From" := (![uint64T] (struct.field_ref raft "id" (![ptrT] "r"))) in
-     let: "Term" := #(W64 0) in
-     let: "Entries" := (![sliceT] "ents") in
-     let: "Responses" := ((let: "$sl0" := (let: "$a0" := (![ptrT] "r") in
+    return: (let: "$Type" := raftpb.MsgStorageApply in
+     let: "$To" := LocalApplyThread in
+     let: "$From" := (![uint64T] (struct.field_ref raft "id" (![ptrT] "r"))) in
+     let: "$Term" := #(W64 0) in
+     let: "$Entries" := (![sliceT] "ents") in
+     let: "$Responses" := ((let: "$sl0" := (let: "$a0" := (![ptrT] "r") in
      let: "$a1" := (![sliceT] "ents") in
      newStorageApplyRespMsg "$a0" "$a1") in
      slice.literal raftpb.Message ["$sl0"])) in
      struct.make raftpb.Message [{
-       "Type" ::= "Type";
-       "To" ::= "To";
-       "From" ::= "From";
-       "Term" ::= "Term";
+       "Type" ::= "$Type";
+       "To" ::= "$To";
+       "From" ::= "$From";
+       "Term" ::= "$Term";
        "LogTerm" ::= zero_val uint64T;
        "Index" ::= zero_val uint64T;
-       "Entries" ::= "Entries";
+       "Entries" ::= "$Entries";
        "Commit" ::= zero_val uint64T;
        "Vote" ::= zero_val uint64T;
        "Snapshot" ::= zero_val ptrT;
        "Reject" ::= zero_val boolT;
        "RejectHint" ::= zero_val uint64T;
        "Context" ::= zero_val sliceT;
-       "Responses" ::= "Responses"
+       "Responses" ::= "$Responses"
      }])).
 
 (* go: rawnode.go:202:6 *)
@@ -4949,18 +4949,18 @@ Definition newStorageAppendMsg : val :=
     exception_do (let: "rd" := (ref_ty Ready "rd") in
     let: "r" := (ref_ty ptrT "r") in
     let: "m" := (ref_ty raftpb.Message (zero_val raftpb.Message)) in
-    let: "$r0" := (let: "Type" := raftpb.MsgStorageAppend in
-    let: "To" := LocalAppendThread in
-    let: "From" := (![uint64T] (struct.field_ref raft "id" (![ptrT] "r"))) in
-    let: "Entries" := (![sliceT] (struct.field_ref Ready "Entries" "rd")) in
+    let: "$r0" := (let: "$Type" := raftpb.MsgStorageAppend in
+    let: "$To" := LocalAppendThread in
+    let: "$From" := (![uint64T] (struct.field_ref raft "id" (![ptrT] "r"))) in
+    let: "$Entries" := (![sliceT] (struct.field_ref Ready "Entries" "rd")) in
     struct.make raftpb.Message [{
-      "Type" ::= "Type";
-      "To" ::= "To";
-      "From" ::= "From";
+      "Type" ::= "$Type";
+      "To" ::= "$To";
+      "From" ::= "$From";
       "Term" ::= zero_val uint64T;
       "LogTerm" ::= zero_val uint64T;
       "Index" ::= zero_val uint64T;
-      "Entries" ::= "Entries";
+      "Entries" ::= "$Entries";
       "Commit" ::= zero_val uint64T;
       "Vote" ::= zero_val uint64T;
       "Snapshot" ::= zero_val ptrT;
@@ -5027,18 +5027,18 @@ Definition RawNode__readyWithoutAccept : val :=
     let: "$r0" := (![ptrT] (struct.field_ref RawNode "raft" (![ptrT] "rn"))) in
     do:  ("r" <-[ptrT] "$r0");;;
     let: "rd" := (ref_ty Ready (zero_val Ready)) in
-    let: "$r0" := (let: "Entries" := ((raftLog__nextUnstableEnts (![ptrT] (struct.field_ref raft "raftLog" (![ptrT] "r")))) #()) in
-    let: "CommittedEntries" := (let: "$a0" := ((RawNode__applyUnstableEntries (![ptrT] "rn")) #()) in
+    let: "$r0" := (let: "$Entries" := ((raftLog__nextUnstableEnts (![ptrT] (struct.field_ref raft "raftLog" (![ptrT] "r")))) #()) in
+    let: "$CommittedEntries" := (let: "$a0" := ((RawNode__applyUnstableEntries (![ptrT] "rn")) #()) in
     (raftLog__nextCommittedEnts (![ptrT] (struct.field_ref raft "raftLog" (![ptrT] "r")))) "$a0") in
-    let: "Messages" := (![sliceT] (struct.field_ref raft "msgs" (![ptrT] "r"))) in
+    let: "$Messages" := (![sliceT] (struct.field_ref raft "msgs" (![ptrT] "r"))) in
     struct.make Ready [{
       "SoftState" ::= zero_val ptrT;
       "HardState" ::= zero_val raftpb.HardState;
       "ReadStates" ::= zero_val sliceT;
-      "Entries" ::= "Entries";
+      "Entries" ::= "$Entries";
       "Snapshot" ::= zero_val raftpb.Snapshot;
-      "CommittedEntries" ::= "CommittedEntries";
-      "Messages" ::= "Messages";
+      "CommittedEntries" ::= "$CommittedEntries";
+      "Messages" ::= "$Messages";
       "MustSync" ::= zero_val boolT
     }]) in
     do:  ("rd" <-[Ready] "$r0");;;
@@ -5581,16 +5581,16 @@ Definition raft__appendEntry : val :=
     let: "$r0" := (let: "$a0" := (![sliceT] "es") in
     (raftLog__append (![ptrT] (struct.field_ref raft "raftLog" (![ptrT] "r")))) "$a0") in
     do:  ("li" <-[uint64T] "$r0");;;
-    do:  (let: "$a0" := (let: "To" := (![uint64T] (struct.field_ref raft "id" (![ptrT] "r"))) in
-    let: "Type" := raftpb.MsgAppResp in
-    let: "Index" := (![uint64T] "li") in
+    do:  (let: "$a0" := (let: "$To" := (![uint64T] (struct.field_ref raft "id" (![ptrT] "r"))) in
+    let: "$Type" := raftpb.MsgAppResp in
+    let: "$Index" := (![uint64T] "li") in
     struct.make raftpb.Message [{
-      "Type" ::= "Type";
-      "To" ::= "To";
+      "Type" ::= "$Type";
+      "To" ::= "$To";
       "From" ::= zero_val uint64T;
       "Term" ::= zero_val uint64T;
       "LogTerm" ::= zero_val uint64T;
-      "Index" ::= "Index";
+      "Index" ::= "$Index";
       "Entries" ::= zero_val sliceT;
       "Commit" ::= zero_val uint64T;
       "Vote" ::= zero_val uint64T;
@@ -5619,24 +5619,24 @@ Definition raft__sendHeartbeat : val :=
     let: "$a1" := (![uint64T] (struct.field_ref raftLog "committed" (![ptrT] (struct.field_ref raft "raftLog" (![ptrT] "r"))))) in
     (minUint64 2) "$a0" "$a1") in
     do:  ("commit" <-[uint64T] "$r0");;;
-    do:  (let: "$a0" := (let: "To" := (![uint64T] "to") in
-    let: "Type" := raftpb.MsgHeartbeat in
-    let: "Commit" := (![uint64T] "commit") in
-    let: "Context" := (![sliceT] "ctx") in
+    do:  (let: "$a0" := (let: "$To" := (![uint64T] "to") in
+    let: "$Type" := raftpb.MsgHeartbeat in
+    let: "$Commit" := (![uint64T] "commit") in
+    let: "$Context" := (![sliceT] "ctx") in
     struct.make raftpb.Message [{
-      "Type" ::= "Type";
-      "To" ::= "To";
+      "Type" ::= "$Type";
+      "To" ::= "$To";
       "From" ::= zero_val uint64T;
       "Term" ::= zero_val uint64T;
       "LogTerm" ::= zero_val uint64T;
       "Index" ::= zero_val uint64T;
       "Entries" ::= zero_val sliceT;
-      "Commit" ::= "Commit";
+      "Commit" ::= "$Commit";
       "Vote" ::= zero_val uint64T;
       "Snapshot" ::= zero_val ptrT;
       "Reject" ::= zero_val boolT;
       "RejectHint" ::= zero_val uint64T;
-      "Context" ::= "Context";
+      "Context" ::= "$Context";
       "Responses" ::= zero_val sliceT
     }]) in
     (raft__send (![ptrT] "r")) "$a0");;;
@@ -5728,12 +5728,12 @@ Definition raft__becomeLeader : val :=
     do:  (let: "$a0" := (![ptrT] "r") in
     traceBecomeLeader "$a0");;;
     let: "emptyEnt" := (ref_ty raftpb.Entry (zero_val raftpb.Entry)) in
-    let: "$r0" := (let: "Data" := #slice.nil in
+    let: "$r0" := (let: "$Data" := #slice.nil in
     struct.make raftpb.Entry [{
       "Term" ::= zero_val uint64T;
       "Index" ::= zero_val uint64T;
       "Type" ::= zero_val raftpb.EntryType;
-      "Data" ::= "Data"
+      "Data" ::= "$Data"
     }]) in
     do:  ("emptyEnt" <-[raftpb.Entry] "$r0");;;
     (if: (~ (let: "$a0" := ((let: "$sl0" := (![raftpb.Entry] "emptyEnt") in
@@ -5768,18 +5768,18 @@ Definition raft__committedEntryInCurrentTerm : val :=
 Definition logSliceFromMsgApp : val :=
   rec: "logSliceFromMsgApp" "m" :=
     exception_do (let: "m" := (ref_ty ptrT "m") in
-    return: (let: "term" := (![uint64T] (struct.field_ref raftpb.Message "Term" (![ptrT] "m"))) in
-     let: "prev" := (let: "term" := (![uint64T] (struct.field_ref raftpb.Message "LogTerm" (![ptrT] "m"))) in
-     let: "index" := (![uint64T] (struct.field_ref raftpb.Message "Index" (![ptrT] "m"))) in
+    return: (let: "$term" := (![uint64T] (struct.field_ref raftpb.Message "Term" (![ptrT] "m"))) in
+     let: "$prev" := (let: "$term" := (![uint64T] (struct.field_ref raftpb.Message "LogTerm" (![ptrT] "m"))) in
+     let: "$index" := (![uint64T] (struct.field_ref raftpb.Message "Index" (![ptrT] "m"))) in
      struct.make entryID [{
-       "term" ::= "term";
-       "index" ::= "index"
+       "term" ::= "$term";
+       "index" ::= "$index"
      }]) in
-     let: "entries" := (![sliceT] (struct.field_ref raftpb.Message "Entries" (![ptrT] "m"))) in
+     let: "$entries" := (![sliceT] (struct.field_ref raftpb.Message "Entries" (![ptrT] "m"))) in
      struct.make logSlice [{
-       "term" ::= "term";
-       "prev" ::= "prev";
-       "entries" ::= "entries"
+       "term" ::= "$term";
+       "prev" ::= "$prev";
+       "entries" ::= "$entries"
      }])).
 
 (* go: raft.go:1811:16 *)
@@ -5793,16 +5793,16 @@ Definition raft__handleAppendEntries : val :=
     do:  ("a" <-[logSlice] "$r0");;;
     (if: (![uint64T] (struct.field_ref entryID "index" (struct.field_ref logSlice "prev" "a"))) < (![uint64T] (struct.field_ref raftLog "committed" (![ptrT] (struct.field_ref raft "raftLog" (![ptrT] "r")))))
     then
-      do:  (let: "$a0" := (let: "To" := (![uint64T] (struct.field_ref raftpb.Message "From" "m")) in
-      let: "Type" := raftpb.MsgAppResp in
-      let: "Index" := (![uint64T] (struct.field_ref raftLog "committed" (![ptrT] (struct.field_ref raft "raftLog" (![ptrT] "r"))))) in
+      do:  (let: "$a0" := (let: "$To" := (![uint64T] (struct.field_ref raftpb.Message "From" "m")) in
+      let: "$Type" := raftpb.MsgAppResp in
+      let: "$Index" := (![uint64T] (struct.field_ref raftLog "committed" (![ptrT] (struct.field_ref raft "raftLog" (![ptrT] "r"))))) in
       struct.make raftpb.Message [{
-        "Type" ::= "Type";
-        "To" ::= "To";
+        "Type" ::= "$Type";
+        "To" ::= "$To";
         "From" ::= zero_val uint64T;
         "Term" ::= zero_val uint64T;
         "LogTerm" ::= zero_val uint64T;
-        "Index" ::= "Index";
+        "Index" ::= "$Index";
         "Entries" ::= zero_val sliceT;
         "Commit" ::= zero_val uint64T;
         "Vote" ::= zero_val uint64T;
@@ -5826,16 +5826,16 @@ Definition raft__handleAppendEntries : val :=
     do:  ("ok" <-[boolT] "$r1");;;
     (if: ![boolT] "ok"
     then
-      do:  (let: "$a0" := (let: "To" := (![uint64T] (struct.field_ref raftpb.Message "From" "m")) in
-      let: "Type" := raftpb.MsgAppResp in
-      let: "Index" := (![uint64T] "mlastIndex") in
+      do:  (let: "$a0" := (let: "$To" := (![uint64T] (struct.field_ref raftpb.Message "From" "m")) in
+      let: "$Type" := raftpb.MsgAppResp in
+      let: "$Index" := (![uint64T] "mlastIndex") in
       struct.make raftpb.Message [{
-        "Type" ::= "Type";
-        "To" ::= "To";
+        "Type" ::= "$Type";
+        "To" ::= "$To";
         "From" ::= zero_val uint64T;
         "Term" ::= zero_val uint64T;
         "LogTerm" ::= zero_val uint64T;
-        "Index" ::= "Index";
+        "Index" ::= "$Index";
         "Entries" ::= zero_val sliceT;
         "Commit" ::= zero_val uint64T;
         "Vote" ::= zero_val uint64T;
@@ -5874,25 +5874,25 @@ Definition raft__handleAppendEntries : val :=
     let: "$r1" := "$ret1" in
     do:  ("hintIndex" <-[uint64T] "$r0");;;
     do:  ("hintTerm" <-[uint64T] "$r1");;;
-    do:  (let: "$a0" := (let: "To" := (![uint64T] (struct.field_ref raftpb.Message "From" "m")) in
-    let: "Type" := raftpb.MsgAppResp in
-    let: "Index" := (![uint64T] (struct.field_ref raftpb.Message "Index" "m")) in
-    let: "Reject" := #true in
-    let: "RejectHint" := (![uint64T] "hintIndex") in
-    let: "LogTerm" := (![uint64T] "hintTerm") in
+    do:  (let: "$a0" := (let: "$To" := (![uint64T] (struct.field_ref raftpb.Message "From" "m")) in
+    let: "$Type" := raftpb.MsgAppResp in
+    let: "$Index" := (![uint64T] (struct.field_ref raftpb.Message "Index" "m")) in
+    let: "$Reject" := #true in
+    let: "$RejectHint" := (![uint64T] "hintIndex") in
+    let: "$LogTerm" := (![uint64T] "hintTerm") in
     struct.make raftpb.Message [{
-      "Type" ::= "Type";
-      "To" ::= "To";
+      "Type" ::= "$Type";
+      "To" ::= "$To";
       "From" ::= zero_val uint64T;
       "Term" ::= zero_val uint64T;
-      "LogTerm" ::= "LogTerm";
-      "Index" ::= "Index";
+      "LogTerm" ::= "$LogTerm";
+      "Index" ::= "$Index";
       "Entries" ::= zero_val sliceT;
       "Commit" ::= zero_val uint64T;
       "Vote" ::= zero_val uint64T;
       "Snapshot" ::= zero_val ptrT;
-      "Reject" ::= "Reject";
-      "RejectHint" ::= "RejectHint";
+      "Reject" ::= "$Reject";
+      "RejectHint" ::= "$RejectHint";
       "Context" ::= zero_val sliceT;
       "Responses" ::= zero_val sliceT
     }]) in
@@ -5905,12 +5905,12 @@ Definition raft__handleHeartbeat : val :=
     let: "m" := (ref_ty raftpb.Message "m") in
     do:  (let: "$a0" := (![uint64T] (struct.field_ref raftpb.Message "Commit" "m")) in
     (raftLog__commitTo (![ptrT] (struct.field_ref raft "raftLog" (![ptrT] "r")))) "$a0");;;
-    do:  (let: "$a0" := (let: "To" := (![uint64T] (struct.field_ref raftpb.Message "From" "m")) in
-    let: "Type" := raftpb.MsgHeartbeatResp in
-    let: "Context" := (![sliceT] (struct.field_ref raftpb.Message "Context" "m")) in
+    do:  (let: "$a0" := (let: "$To" := (![uint64T] (struct.field_ref raftpb.Message "From" "m")) in
+    let: "$Type" := raftpb.MsgHeartbeatResp in
+    let: "$Context" := (![sliceT] (struct.field_ref raftpb.Message "Context" "m")) in
     struct.make raftpb.Message [{
-      "Type" ::= "Type";
-      "To" ::= "To";
+      "Type" ::= "$Type";
+      "To" ::= "$To";
       "From" ::= zero_val uint64T;
       "Term" ::= zero_val uint64T;
       "LogTerm" ::= zero_val uint64T;
@@ -5921,7 +5921,7 @@ Definition raft__handleHeartbeat : val :=
       "Snapshot" ::= zero_val ptrT;
       "Reject" ::= zero_val boolT;
       "RejectHint" ::= zero_val uint64T;
-      "Context" ::= "Context";
+      "Context" ::= "$Context";
       "Responses" ::= zero_val sliceT
     }]) in
     (raft__send (![ptrT] "r")) "$a0")).
@@ -5983,11 +5983,11 @@ Definition raft__restore : val :=
       return: (#false)
     else do:  #());;;
     let: "id" := (ref_ty entryID (zero_val entryID)) in
-    let: "$r0" := (let: "term" := (![uint64T] (struct.field_ref raftpb.SnapshotMetadata "Term" (struct.field_ref raftpb.Snapshot "Metadata" "s"))) in
-    let: "index" := (![uint64T] (struct.field_ref raftpb.SnapshotMetadata "Index" (struct.field_ref raftpb.Snapshot "Metadata" "s"))) in
+    let: "$r0" := (let: "$term" := (![uint64T] (struct.field_ref raftpb.SnapshotMetadata "Term" (struct.field_ref raftpb.Snapshot "Metadata" "s"))) in
+    let: "$index" := (![uint64T] (struct.field_ref raftpb.SnapshotMetadata "Index" (struct.field_ref raftpb.Snapshot "Metadata" "s"))) in
     struct.make entryID [{
-      "term" ::= "term";
-      "index" ::= "index"
+      "term" ::= "$term";
+      "index" ::= "$index"
     }]) in
     do:  ("id" <-[entryID] "$r0");;;
     (if: let: "$a0" := (![entryID] "id") in
@@ -6018,11 +6018,11 @@ Definition raft__restore : val :=
     let: "err" := (ref_ty error (zero_val error)) in
     let: "trk" := (ref_ty tracker.ProgressMap (zero_val tracker.ProgressMap)) in
     let: "cfg" := (ref_ty tracker.Config (zero_val tracker.Config)) in
-    let: (("$ret0", "$ret1"), "$ret2") := (let: "$a0" := (let: "Tracker" := (![tracker.ProgressTracker] (struct.field_ref raft "trk" (![ptrT] "r"))) in
-    let: "LastIndex" := ((raftLog__lastIndex (![ptrT] (struct.field_ref raft "raftLog" (![ptrT] "r")))) #()) in
+    let: (("$ret0", "$ret1"), "$ret2") := (let: "$a0" := (let: "$Tracker" := (![tracker.ProgressTracker] (struct.field_ref raft "trk" (![ptrT] "r"))) in
+    let: "$LastIndex" := ((raftLog__lastIndex (![ptrT] (struct.field_ref raft "raftLog" (![ptrT] "r")))) #()) in
     struct.make confchange.Changer [{
-      "Tracker" ::= "Tracker";
-      "LastIndex" ::= "LastIndex"
+      "Tracker" ::= "$Tracker";
+      "LastIndex" ::= "$LastIndex"
     }]) in
     let: "$a1" := (![raftpb.ConfState] "cs") in
     confchange.Restore "$a0" "$a1") in
@@ -6088,16 +6088,16 @@ Definition raft__handleSnapshot : val :=
       let: "$sl3" := (interface.make uint64__mset (![uint64T] "sterm")) in
       slice.literal interfaceT ["$sl0"; "$sl1"; "$sl2"; "$sl3"])) in
       (interface.get "Infof" (![Logger] (struct.field_ref raft "logger" (![ptrT] "r")))) "$a0" "$a1");;;
-      do:  (let: "$a0" := (let: "To" := (![uint64T] (struct.field_ref raftpb.Message "From" "m")) in
-      let: "Type" := raftpb.MsgAppResp in
-      let: "Index" := ((raftLog__lastIndex (![ptrT] (struct.field_ref raft "raftLog" (![ptrT] "r")))) #()) in
+      do:  (let: "$a0" := (let: "$To" := (![uint64T] (struct.field_ref raftpb.Message "From" "m")) in
+      let: "$Type" := raftpb.MsgAppResp in
+      let: "$Index" := ((raftLog__lastIndex (![ptrT] (struct.field_ref raft "raftLog" (![ptrT] "r")))) #()) in
       struct.make raftpb.Message [{
-        "Type" ::= "Type";
-        "To" ::= "To";
+        "Type" ::= "$Type";
+        "To" ::= "$To";
         "From" ::= zero_val uint64T;
         "Term" ::= zero_val uint64T;
         "LogTerm" ::= zero_val uint64T;
-        "Index" ::= "Index";
+        "Index" ::= "$Index";
         "Entries" ::= zero_val sliceT;
         "Commit" ::= zero_val uint64T;
         "Vote" ::= zero_val uint64T;
@@ -6116,16 +6116,16 @@ Definition raft__handleSnapshot : val :=
       let: "$sl3" := (interface.make uint64__mset (![uint64T] "sterm")) in
       slice.literal interfaceT ["$sl0"; "$sl1"; "$sl2"; "$sl3"])) in
       (interface.get "Infof" (![Logger] (struct.field_ref raft "logger" (![ptrT] "r")))) "$a0" "$a1");;;
-      do:  (let: "$a0" := (let: "To" := (![uint64T] (struct.field_ref raftpb.Message "From" "m")) in
-      let: "Type" := raftpb.MsgAppResp in
-      let: "Index" := (![uint64T] (struct.field_ref raftLog "committed" (![ptrT] (struct.field_ref raft "raftLog" (![ptrT] "r"))))) in
+      do:  (let: "$a0" := (let: "$To" := (![uint64T] (struct.field_ref raftpb.Message "From" "m")) in
+      let: "$Type" := raftpb.MsgAppResp in
+      let: "$Index" := (![uint64T] (struct.field_ref raftLog "committed" (![ptrT] (struct.field_ref raft "raftLog" (![ptrT] "r"))))) in
       struct.make raftpb.Message [{
-        "Type" ::= "Type";
-        "To" ::= "To";
+        "Type" ::= "$Type";
+        "To" ::= "$To";
         "From" ::= zero_val uint64T;
         "Term" ::= zero_val uint64T;
         "LogTerm" ::= zero_val uint64T;
-        "Index" ::= "Index";
+        "Index" ::= "$Index";
         "Entries" ::= zero_val sliceT;
         "Commit" ::= zero_val uint64T;
         "Vote" ::= zero_val uint64T;
@@ -6193,11 +6193,11 @@ Definition raft__responseToReadIndexReq : val :=
     (if: ((![uint64T] (struct.field_ref raftpb.Message "From" "req")) = None) || ((![uint64T] (struct.field_ref raftpb.Message "From" "req")) = (![uint64T] (struct.field_ref raft "id" (![ptrT] "r"))))
     then
       let: "$r0" := (let: "$a0" := (![sliceT] (struct.field_ref raft "readStates" (![ptrT] "r"))) in
-      let: "$a1" := ((let: "$sl0" := (let: "Index" := (![uint64T] "readIndex") in
-      let: "RequestCtx" := (![sliceT] (struct.field_ref raftpb.Entry "Data" (slice.elem_ref raftpb.Entry (![sliceT] (struct.field_ref raftpb.Message "Entries" "req")) #(W64 0)))) in
+      let: "$a1" := ((let: "$sl0" := (let: "$Index" := (![uint64T] "readIndex") in
+      let: "$RequestCtx" := (![sliceT] (struct.field_ref raftpb.Entry "Data" (slice.elem_ref raftpb.Entry (![sliceT] (struct.field_ref raftpb.Message "Entries" "req")) #(W64 0)))) in
       struct.make ReadState [{
-        "Index" ::= "Index";
-        "RequestCtx" ::= "RequestCtx"
+        "Index" ::= "$Index";
+        "RequestCtx" ::= "$RequestCtx"
       }]) in
       slice.literal ReadState ["$sl0"])) in
       (slice.append sliceT) "$a0" "$a1") in
@@ -6219,18 +6219,18 @@ Definition raft__responseToReadIndexReq : val :=
          "Responses" ::= zero_val sliceT
        }])
     else do:  #());;;
-    return: (let: "Type" := raftpb.MsgReadIndexResp in
-     let: "To" := (![uint64T] (struct.field_ref raftpb.Message "From" "req")) in
-     let: "Index" := (![uint64T] "readIndex") in
-     let: "Entries" := (![sliceT] (struct.field_ref raftpb.Message "Entries" "req")) in
+    return: (let: "$Type" := raftpb.MsgReadIndexResp in
+     let: "$To" := (![uint64T] (struct.field_ref raftpb.Message "From" "req")) in
+     let: "$Index" := (![uint64T] "readIndex") in
+     let: "$Entries" := (![sliceT] (struct.field_ref raftpb.Message "Entries" "req")) in
      struct.make raftpb.Message [{
-       "Type" ::= "Type";
-       "To" ::= "To";
+       "Type" ::= "$Type";
+       "To" ::= "$To";
        "From" ::= zero_val uint64T;
        "Term" ::= zero_val uint64T;
        "LogTerm" ::= zero_val uint64T;
-       "Index" ::= "Index";
-       "Entries" ::= "Entries";
+       "Index" ::= "$Index";
+       "Entries" ::= "$Entries";
        "Commit" ::= zero_val uint64T;
        "Vote" ::= zero_val uint64T;
        "Snapshot" ::= zero_val ptrT;
@@ -6245,11 +6245,11 @@ Definition raft__sendTimeoutNow : val :=
   rec: "raft__sendTimeoutNow" "r" "to" :=
     exception_do (let: "r" := (ref_ty ptrT "r") in
     let: "to" := (ref_ty uint64T "to") in
-    do:  (let: "$a0" := (let: "To" := (![uint64T] "to") in
-    let: "Type" := raftpb.MsgTimeoutNow in
+    do:  (let: "$a0" := (let: "$To" := (![uint64T] "to") in
+    let: "$Type" := raftpb.MsgTimeoutNow in
     struct.make raftpb.Message [{
-      "Type" ::= "Type";
-      "To" ::= "To";
+      "Type" ::= "$Type";
+      "To" ::= "$To";
       "From" ::= zero_val uint64T;
       "Term" ::= zero_val uint64T;
       "LogTerm" ::= zero_val uint64T;
@@ -6434,13 +6434,13 @@ Definition readOnly__addRequest : val :=
     (if: ![boolT] "ok"
     then return: (#())
     else do:  #()));;;
-    let: "$r0" := (ref_ty readIndexStatus (let: "index" := (![uint64T] "index") in
-    let: "req" := (![raftpb.Message] "m") in
-    let: "acks" := (map.make uint64T boolT #()) in
+    let: "$r0" := (ref_ty readIndexStatus (let: "$index" := (![uint64T] "index") in
+    let: "$req" := (![raftpb.Message] "m") in
+    let: "$acks" := (map.make uint64T boolT #()) in
     struct.make readIndexStatus [{
-      "req" ::= "req";
-      "index" ::= "index";
-      "acks" ::= "acks"
+      "req" ::= "$req";
+      "index" ::= "$index";
+      "acks" ::= "$acks"
     }])) in
     do:  (map.insert (![mapT stringT ptrT] (struct.field_ref readOnly "pendingReadIndex" (![ptrT] "ro"))) (![stringT] "s") "$r0");;;
     let: "$r0" := (let: "$a0" := (![sliceT] (struct.field_ref readOnly "readIndexQueue" (![ptrT] "ro"))) in
@@ -6651,11 +6651,11 @@ Definition stepLeader : val :=
                 let: "$sl3" := (interface.make string__mset (![stringT] "failedCheck")) in
                 slice.literal interfaceT ["$sl0"; "$sl1"; "$sl2"; "$sl3"])) in
                 (interface.get "Infof" (![Logger] (struct.field_ref raft "logger" (![ptrT] "r")))) "$a0" "$a1");;;
-                let: "$r0" := (let: "Type" := raftpb.EntryNormal in
+                let: "$r0" := (let: "$Type" := raftpb.EntryNormal in
                 struct.make raftpb.Entry [{
                   "Term" ::= zero_val uint64T;
                   "Index" ::= zero_val uint64T;
-                  "Type" ::= "Type";
+                  "Type" ::= "$Type";
                   "Data" ::= zero_val sliceT
                 }]) in
                 do:  ((slice.elem_ref raftpb.Entry (![sliceT] (struct.field_ref raftpb.Message "Entries" "m")) (![intT] "i")) <-[raftpb.Entry] "$r0")
@@ -7206,11 +7206,11 @@ Definition stepFollower : val :=
                         return: (#interface.nil)
                       else do:  #());;;
                       let: "$r0" := (let: "$a0" := (![sliceT] (struct.field_ref raft "readStates" (![ptrT] "r"))) in
-                      let: "$a1" := ((let: "$sl0" := (let: "Index" := (![uint64T] (struct.field_ref raftpb.Message "Index" "m")) in
-                      let: "RequestCtx" := (![sliceT] (struct.field_ref raftpb.Entry "Data" (slice.elem_ref raftpb.Entry (![sliceT] (struct.field_ref raftpb.Message "Entries" "m")) #(W64 0)))) in
+                      let: "$a1" := ((let: "$sl0" := (let: "$Index" := (![uint64T] (struct.field_ref raftpb.Message "Index" "m")) in
+                      let: "$RequestCtx" := (![sliceT] (struct.field_ref raftpb.Entry "Data" (slice.elem_ref raftpb.Entry (![sliceT] (struct.field_ref raftpb.Message "Entries" "m")) #(W64 0)))) in
                       struct.make ReadState [{
-                        "Index" ::= "Index";
-                        "RequestCtx" ::= "RequestCtx"
+                        "Index" ::= "$Index";
+                        "RequestCtx" ::= "$RequestCtx"
                       }]) in
                       slice.literal ReadState ["$sl0"])) in
                       (slice.append sliceT) "$a0" "$a1") in
@@ -7235,23 +7235,23 @@ Definition newTestConfig : val :=
     let: "heartbeat" := (ref_ty intT "heartbeat") in
     let: "election" := (ref_ty intT "election") in
     let: "id" := (ref_ty uint64T "id") in
-    return: (ref_ty Config (let: "ID" := (![uint64T] "id") in
-     let: "ElectionTick" := (![intT] "election") in
-     let: "HeartbeatTick" := (![intT] "heartbeat") in
-     let: "Storage" := (![Storage] "storage") in
-     let: "MaxSizePerMsg" := #(W64 noLimit) in
-     let: "MaxInflightMsgs" := #(W64 256) in
+    return: (ref_ty Config (let: "$ID" := (![uint64T] "id") in
+     let: "$ElectionTick" := (![intT] "election") in
+     let: "$HeartbeatTick" := (![intT] "heartbeat") in
+     let: "$Storage" := (![Storage] "storage") in
+     let: "$MaxSizePerMsg" := #(W64 noLimit) in
+     let: "$MaxInflightMsgs" := #(W64 256) in
      struct.make Config [{
-       "ID" ::= "ID";
-       "ElectionTick" ::= "ElectionTick";
-       "HeartbeatTick" ::= "HeartbeatTick";
-       "Storage" ::= "Storage";
+       "ID" ::= "$ID";
+       "ElectionTick" ::= "$ElectionTick";
+       "HeartbeatTick" ::= "$HeartbeatTick";
+       "Storage" ::= "$Storage";
        "Applied" ::= zero_val uint64T;
        "AsyncStorageWrites" ::= zero_val boolT;
-       "MaxSizePerMsg" ::= "MaxSizePerMsg";
+       "MaxSizePerMsg" ::= "$MaxSizePerMsg";
        "MaxCommittedSizePerReady" ::= zero_val uint64T;
        "MaxUncommittedEntriesSize" ::= zero_val uint64T;
-       "MaxInflightMsgs" ::= "MaxInflightMsgs";
+       "MaxInflightMsgs" ::= "$MaxInflightMsgs";
        "MaxInflightBytes" ::= zero_val uint64T;
        "CheckQuorum" ::= zero_val boolT;
        "PreVote" ::= zero_val boolT;
@@ -7383,11 +7383,11 @@ Definition MemoryStorage__ApplySnapshot : val :=
     else do:  #());;;
     let: "$r0" := (![raftpb.Snapshot] "snap") in
     do:  ((struct.field_ref MemoryStorage "snapshot" (![ptrT] "ms")) <-[raftpb.Snapshot] "$r0");;;
-    let: "$r0" := ((let: "$sl0" := (let: "Term" := (![uint64T] (struct.field_ref raftpb.SnapshotMetadata "Term" (struct.field_ref raftpb.Snapshot "Metadata" "snap"))) in
-    let: "Index" := (![uint64T] (struct.field_ref raftpb.SnapshotMetadata "Index" (struct.field_ref raftpb.Snapshot "Metadata" "snap"))) in
+    let: "$r0" := ((let: "$sl0" := (let: "$Term" := (![uint64T] (struct.field_ref raftpb.SnapshotMetadata "Term" (struct.field_ref raftpb.Snapshot "Metadata" "snap"))) in
+    let: "$Index" := (![uint64T] (struct.field_ref raftpb.SnapshotMetadata "Index" (struct.field_ref raftpb.Snapshot "Metadata" "snap"))) in
     struct.make raftpb.Entry [{
-      "Term" ::= "Term";
-      "Index" ::= "Index";
+      "Term" ::= "$Term";
+      "Index" ::= "$Index";
       "Type" ::= zero_val raftpb.EntryType;
       "Data" ::= zero_val sliceT
     }]) in
@@ -7673,12 +7673,12 @@ Definition MemoryStorage__mset_ptr : list (string * val) := [
    go: storage.go:113:6 *)
 Definition NewMemoryStorage : val :=
   rec: "NewMemoryStorage" <> :=
-    exception_do (return: (ref_ty MemoryStorage (let: "ents" := (slice.make2 raftpb.Entry #(W64 1)) in
+    exception_do (return: (ref_ty MemoryStorage (let: "$ents" := (slice.make2 raftpb.Entry #(W64 1)) in
      struct.make MemoryStorage [{
        "Mutex" ::= zero_val sync.Mutex;
        "hardState" ::= zero_val raftpb.HardState;
        "snapshot" ::= zero_val raftpb.Snapshot;
-       "ents" ::= "ents";
+       "ents" ::= "$ents";
        "callStats" ::= zero_val inMemStorageCallStats
      }]))).
 
@@ -7694,11 +7694,11 @@ Definition entsWithConfig : val :=
     slice.for_range uint64T "$range" (λ: "i" "term",
       let: "i" := ref_ty uint64T "i" in
       let: "term" := ref_ty uint64T "term" in
-      do:  (let: "$a0" := ((let: "$sl0" := (let: "Index" := ((![intT] "i") + #(W64 1)) in
-      let: "Term" := (![uint64T] "term") in
+      do:  (let: "$a0" := ((let: "$sl0" := (let: "$Index" := ((![intT] "i") + #(W64 1)) in
+      let: "$Term" := (![uint64T] "term") in
       struct.make raftpb.Entry [{
-        "Term" ::= "Term";
-        "Index" ::= "Index";
+        "Term" ::= "$Term";
+        "Index" ::= "$Index";
         "Type" ::= zero_val raftpb.EntryType;
         "Data" ::= zero_val sliceT
       }]) in
@@ -8246,16 +8246,16 @@ Definition newNetworkWithConfigInit : val :=
       else
         let: "$r0" := (![stateMachine] "p") in
         do:  (map.insert (![mapT uint64T stateMachine] "npeers") (![uint64T] "id") "$r0"))));;;
-    return: (ref_ty network (let: "peers" := (![mapT uint64T stateMachine] "npeers") in
-     let: "storage" := (![mapT uint64T ptrT] "nstorage") in
-     let: "dropm64" := (map.make connem uint64T #()) in
-     let: "ignorem" := (map.make raftpb.MessageType boolT #()) in
+    return: (ref_ty network (let: "$peers" := (![mapT uint64T stateMachine] "npeers") in
+     let: "$storage" := (![mapT uint64T ptrT] "nstorage") in
+     let: "$dropm64" := (map.make connem uint64T #()) in
+     let: "$ignorem" := (map.make raftpb.MessageType boolT #()) in
      struct.make network [{
        "t" ::= zero_val ptrT;
-       "peers" ::= "peers";
-       "storage" ::= "storage";
-       "dropm64" ::= "dropm64";
-       "ignorem" ::= "ignorem";
+       "peers" ::= "$peers";
+       "storage" ::= "$storage";
+       "dropm64" ::= "$dropm64";
+       "ignorem" ::= "$ignorem";
        "msgHook" ::= zero_val funcT
      }]))).
 
@@ -8378,13 +8378,13 @@ Definition testLeaderElection2 : val :=
     slice.for_range testLeaderElectionStruct "$range" (λ: "i" "tt",
       let: "i" := ref_ty uint64T "i" in
       let: "tt" := ref_ty testLeaderElectionStruct "tt" in
-      do:  (let: "$a0" := ((let: "$sl0" := (let: "From" := #(W64 1) in
-      let: "To" := #(W64 1) in
-      let: "Type" := raftpb.MsgHup in
+      do:  (let: "$a0" := ((let: "$sl0" := (let: "$From" := #(W64 1) in
+      let: "$To" := #(W64 1) in
+      let: "$Type" := raftpb.MsgHup in
       struct.make raftpb.Message [{
-        "Type" ::= "Type";
-        "To" ::= "To";
-        "From" ::= "From";
+        "Type" ::= "$Type";
+        "To" ::= "$To";
+        "From" ::= "$From";
         "Term" ::= zero_val uint64T;
         "LogTerm" ::= zero_val uint64T;
         "Index" ::= zero_val uint64T;
@@ -8451,9 +8451,9 @@ Definition RawNode__BasicStatus : val :=
 Definition RawNode__Campaign : val :=
   rec: "RawNode__Campaign" "rn" <> :=
     exception_do (let: "rn" := (ref_ty ptrT "rn") in
-    return: (let: "$a0" := (let: "Type" := raftpb.MsgHup in
+    return: (let: "$a0" := (let: "$Type" := raftpb.MsgHup in
      struct.make raftpb.Message [{
-       "Type" ::= "Type";
+       "Type" ::= "$Type";
        "To" ::= zero_val uint64T;
        "From" ::= zero_val uint64T;
        "Term" ::= zero_val uint64T;
@@ -8477,9 +8477,9 @@ Definition RawNode__Campaign : val :=
 Definition RawNode__ForgetLeader : val :=
   rec: "RawNode__ForgetLeader" "rn" <> :=
     exception_do (let: "rn" := (ref_ty ptrT "rn") in
-    return: (let: "$a0" := (let: "Type" := raftpb.MsgForgetLeader in
+    return: (let: "$a0" := (let: "$Type" := raftpb.MsgForgetLeader in
      struct.make raftpb.Message [{
-       "Type" ::= "Type";
+       "Type" ::= "$Type";
        "To" ::= zero_val uint64T;
        "From" ::= zero_val uint64T;
        "Term" ::= zero_val uint64T;
@@ -8503,24 +8503,24 @@ Definition RawNode__Propose : val :=
   rec: "RawNode__Propose" "rn" "data" :=
     exception_do (let: "rn" := (ref_ty ptrT "rn") in
     let: "data" := (ref_ty sliceT "data") in
-    return: (let: "$a0" := (let: "Type" := raftpb.MsgProp in
-     let: "From" := (![uint64T] (struct.field_ref raft "id" (![ptrT] (struct.field_ref RawNode "raft" (![ptrT] "rn"))))) in
-     let: "Entries" := ((let: "$sl0" := (let: "Data" := (![sliceT] "data") in
+    return: (let: "$a0" := (let: "$Type" := raftpb.MsgProp in
+     let: "$From" := (![uint64T] (struct.field_ref raft "id" (![ptrT] (struct.field_ref RawNode "raft" (![ptrT] "rn"))))) in
+     let: "$Entries" := ((let: "$sl0" := (let: "$Data" := (![sliceT] "data") in
      struct.make raftpb.Entry [{
        "Term" ::= zero_val uint64T;
        "Index" ::= zero_val uint64T;
        "Type" ::= zero_val raftpb.EntryType;
-       "Data" ::= "Data"
+       "Data" ::= "$Data"
      }]) in
      slice.literal raftpb.Entry ["$sl0"])) in
      struct.make raftpb.Message [{
-       "Type" ::= "Type";
+       "Type" ::= "$Type";
        "To" ::= zero_val uint64T;
-       "From" ::= "From";
+       "From" ::= "$From";
        "Term" ::= zero_val uint64T;
        "LogTerm" ::= zero_val uint64T;
        "Index" ::= zero_val uint64T;
-       "Entries" ::= "Entries";
+       "Entries" ::= "$Entries";
        "Commit" ::= zero_val uint64T;
        "Vote" ::= zero_val uint64T;
        "Snapshot" ::= zero_val ptrT;
@@ -8563,23 +8563,23 @@ Definition RawNode__ReadIndex : val :=
   rec: "RawNode__ReadIndex" "rn" "rctx" :=
     exception_do (let: "rn" := (ref_ty ptrT "rn") in
     let: "rctx" := (ref_ty sliceT "rctx") in
-    let: "$r0" := (let: "$a0" := (let: "Type" := raftpb.MsgReadIndex in
-    let: "Entries" := ((let: "$sl0" := (let: "Data" := (![sliceT] "rctx") in
+    let: "$r0" := (let: "$a0" := (let: "$Type" := raftpb.MsgReadIndex in
+    let: "$Entries" := ((let: "$sl0" := (let: "$Data" := (![sliceT] "rctx") in
     struct.make raftpb.Entry [{
       "Term" ::= zero_val uint64T;
       "Index" ::= zero_val uint64T;
       "Type" ::= zero_val raftpb.EntryType;
-      "Data" ::= "Data"
+      "Data" ::= "$Data"
     }]) in
     slice.literal raftpb.Entry ["$sl0"])) in
     struct.make raftpb.Message [{
-      "Type" ::= "Type";
+      "Type" ::= "$Type";
       "To" ::= zero_val uint64T;
       "From" ::= zero_val uint64T;
       "Term" ::= zero_val uint64T;
       "LogTerm" ::= zero_val uint64T;
       "Index" ::= zero_val uint64T;
-      "Entries" ::= "Entries";
+      "Entries" ::= "$Entries";
       "Commit" ::= zero_val uint64T;
       "Vote" ::= zero_val uint64T;
       "Snapshot" ::= zero_val ptrT;
@@ -8618,13 +8618,13 @@ Definition RawNode__ReportSnapshot : val :=
     let: "rej" := (ref_ty boolT (zero_val boolT)) in
     let: "$r0" := ((![SnapshotStatus] "status") = SnapshotFailure) in
     do:  ("rej" <-[boolT] "$r0");;;
-    let: "$r0" := (let: "$a0" := (let: "Type" := raftpb.MsgSnapStatus in
-    let: "From" := (![uint64T] "id") in
-    let: "Reject" := (![boolT] "rej") in
+    let: "$r0" := (let: "$a0" := (let: "$Type" := raftpb.MsgSnapStatus in
+    let: "$From" := (![uint64T] "id") in
+    let: "$Reject" := (![boolT] "rej") in
     struct.make raftpb.Message [{
-      "Type" ::= "Type";
+      "Type" ::= "$Type";
       "To" ::= zero_val uint64T;
-      "From" ::= "From";
+      "From" ::= "$From";
       "Term" ::= zero_val uint64T;
       "LogTerm" ::= zero_val uint64T;
       "Index" ::= zero_val uint64T;
@@ -8632,7 +8632,7 @@ Definition RawNode__ReportSnapshot : val :=
       "Commit" ::= zero_val uint64T;
       "Vote" ::= zero_val uint64T;
       "Snapshot" ::= zero_val ptrT;
-      "Reject" ::= "Reject";
+      "Reject" ::= "$Reject";
       "RejectHint" ::= zero_val uint64T;
       "Context" ::= zero_val sliceT;
       "Responses" ::= zero_val sliceT
@@ -8647,12 +8647,12 @@ Definition RawNode__ReportUnreachable : val :=
   rec: "RawNode__ReportUnreachable" "rn" "id" :=
     exception_do (let: "rn" := (ref_ty ptrT "rn") in
     let: "id" := (ref_ty uint64T "id") in
-    let: "$r0" := (let: "$a0" := (let: "Type" := raftpb.MsgUnreachable in
-    let: "From" := (![uint64T] "id") in
+    let: "$r0" := (let: "$a0" := (let: "$Type" := raftpb.MsgUnreachable in
+    let: "$From" := (![uint64T] "id") in
     struct.make raftpb.Message [{
-      "Type" ::= "Type";
+      "Type" ::= "$Type";
       "To" ::= zero_val uint64T;
-      "From" ::= "From";
+      "From" ::= "$From";
       "Term" ::= zero_val uint64T;
       "LogTerm" ::= zero_val uint64T;
       "Index" ::= zero_val uint64T;
@@ -8725,12 +8725,12 @@ Definition RawNode__TransferLeader : val :=
   rec: "RawNode__TransferLeader" "rn" "transferee" :=
     exception_do (let: "rn" := (ref_ty ptrT "rn") in
     let: "transferee" := (ref_ty uint64T "transferee") in
-    let: "$r0" := (let: "$a0" := (let: "Type" := raftpb.MsgTransferLeader in
-    let: "From" := (![uint64T] "transferee") in
+    let: "$r0" := (let: "$a0" := (let: "$Type" := raftpb.MsgTransferLeader in
+    let: "$From" := (![uint64T] "transferee") in
     struct.make raftpb.Message [{
-      "Type" ::= "Type";
+      "Type" ::= "$Type";
       "To" ::= zero_val uint64T;
-      "From" ::= "From";
+      "From" ::= "$From";
       "Term" ::= zero_val uint64T;
       "LogTerm" ::= zero_val uint64T;
       "Index" ::= zero_val uint64T;
