new/proof/sync.v
@@ -27,7 +27,7 @@ End Mutex.
 
 Instance into_val_Mutex `{ffi_syntax} : IntoVal Mutex.t :=
   {|
-    to_val_def := λ v, struct.val Mutex [("state" ::= #v.(Mutex.state))]%V
+    to_val_def := λ v, struct.val_aux Mutex [("state" ::= #v.(Mutex.state))]%V
   |}.
 
 Program Instance into_val_typed_Mutex `{ffi_syntax} : IntoValTyped Mutex.t Mutex :=
@@ -35,13 +35,13 @@ Program Instance into_val_typed_Mutex `{ffi_syntax} : IntoValTyped Mutex.t Mutex
 Next Obligation. rewrite to_val_unseal /=. solve_has_go_type. Qed.
 Next Obligation.
   (* FIXME: [solve_zero_val] tactic *)
-  intros. rewrite zero_val_eq to_val_unseal /= struct.val_unseal /=.
+  intros. rewrite zero_val_eq to_val_unseal /= struct.val_aux_unseal /=.
   rewrite zero_val_eq /= !to_val_unseal //.
 Qed.
 Next Obligation.
   (* FIXME: automation for this *)
   rewrite to_val_unseal => ? x y Heq.
-  rewrite /= struct.val_unseal /= in Heq.
+  rewrite /= struct.val_aux_unseal /= in Heq.
   inversion Heq.
   destruct x, y.
   f_equal.
@@ -53,7 +53,7 @@ Final Obligation. solve_decision. Qed.
 Program Instance into_val_struct_Mutex_state `{ffi_syntax} :
   IntoValStructField "state" Mutex Mutex.state.
 Final Obligation.
-intros. by rewrite to_val_unseal /= struct.val_unseal /= to_val_unseal /=.
+intros. by rewrite to_val_unseal /= struct.val_aux_unseal /= to_val_unseal /=.
 Qed.
 
 Section goose_lang.
@@ -98,7 +98,6 @@ Theorem init_Mutex R E m : m ↦# (default_val Mutex.t) -∗ ▷ R ={E}=∗ is_M
 Proof.
   iIntros "Hl HR".
   simpl.
-  (* FIXME: typeclass for relating record projections to struct fields. *)
   iDestruct (struct_fields_split with "Hl") as "Hl".
   { done. }
   { apply _. }
